WIP: proved step case for [pthread_create], hoplefully this works for switch, going to check progress again

concur/ThreadLinkingBack.v
@@ -5,8 +5,6 @@ Require Import ValueAnalysis.
 Require Import MultiLibs CMulti AsmMulti.
 Require Import Extends InjectFootprint CA.
 Require Import CallconvBig Ext Injp CAnew Composition.
-
-
 Require Import ThreadLinking.
 
 Section ConcurSim.
@@ -209,38 +207,9 @@ Section ConcurSim.
      
    End Initial.
 
-
-   Definition empty_worlds {T:Type}: NatMap.t (option T) := NatMap.init None.
-   Definition empty_gworlds {T:Type}: NatMap.t (option T) := NatMap.init None.
-   Definition initial_worlds {T: Type} (w: T) := NatMap.set 1%nat (Some w) empty_worlds.
-   Definition initial_gworlds {T:Type} (w: T) := NatMap.set 1%nat (Some w) empty_gworlds.
    Definition initial_indexs (i: bsim_index) := i :: nil.
-    
-    
-    Definition sig_w_compcert (w: GS.ccworld cc_compcert) : signature :=
-      (snd (fst (snd (snd (snd w))))).
 
-    Definition rs_w_compcert (w: GS.ccworld cc_compcert) : regset :=
-      cajw_rs (fst (snd (snd (snd (snd (snd (w))))))).
-
-    Definition injp_w_compcert (w: GS.ccworld cc_compcert) : injp_world :=
-      cajw_injp (fst (snd (snd (snd (snd (snd (w))))))).
-
-    Definition cainjp_w_compcert (w: GS.ccworld cc_compcert) :=
-      (fst (snd (snd (snd (snd (snd (w))))))).
-    
-    Definition regset_lessdef (rs1 rs2: regset) := forall r, Val.lessdef (rs1 r) (rs2 r).
-
-
-    Definition injp_gw_compcert (w: GS.gworld cc_compcert) : injp_world :=
-      fst (snd (snd (w))).
-
-    Inductive wt_w_compcert : GS.ccworld cc_compcert -> Prop :=
-      wt_w_intro : forall se j m1 m2 m3 (tse: Genv.symtbl) sig Hmj Hme rs,
-          wt_w_compcert
-            (se, (row se m1, (se,(se,sig,(tse,(cajw (injpw j m1 m2 Hmj) sig rs, extw m2 m3 Hme)))))).
-
-    Inductive match_thread_states : GS.ccworld cc_compcert -> (option (GS.ccworld cc_compcert)) -> GS.gworld cc_compcert -> bsim_index -> thread_state_C -> thread_state_A -> Prop :=
+   Inductive match_thread_states : GS.ccworld cc_compcert -> (option (GS.ccworld cc_compcert)) -> GS.gworld cc_compcert -> bsim_index -> thread_state_C -> thread_state_A -> Prop :=
     |match_local : forall wB i sc sa wp
         (M_STATES: match_local_states wB wp i sc sa),
         match_thread_states wB None wp i (CMulti.Local OpenC sc) (Local OpenA sa)
@@ -283,37 +252,6 @@ Section ConcurSim.
       (* the signature for all sub threads are start_routine_sig *)
       match_thread_states wB None wp i (CMulti.Final OpenC res) (Final OpenA tres).
 
-
-      
-    Definition injp_tid (w: injp_world) : nat :=
-     match w with injpw j m tm Hm => Mem.tid (Mem.support m) end.
-                     
-    Definition injp_nexttid (w: injp_world) : nat :=
-      match w with injpw j m tm Hm => Mem.next_tid (Mem.support m) end.
-
-    Definition gw_tid (gw: GS.gworld cc_compcert) : nat :=
-      injp_tid (injp_gw_compcert gw).
-
-    Definition gw_nexttid gw : nat := injp_nexttid (injp_gw_compcert gw).
-
-    Inductive gw_accg : GS.gworld cc_compcert -> GS.gworld cc_compcert -> Prop :=
-      gw_accg_intro : forall j m1 m2 j' m1' m2' Hmj Hmj' m3 Hme m3' Hme',
-         injp_accg (injpw j m1 m2 Hmj) (injpw j' m1' m2' Hmj') ->
-         ext_accg (extw m2 m3 Hme) (extw m2' m3' Hme') ->
-         gw_accg (tt,(tt,(injpw j m1 m2 Hmj, extw m2 m3 Hme)))
-           (tt,(tt,(injpw j' m1' m2' Hmj', extw m2' m3' Hme'))).
-
-    Lemma gw_accg_neq : forall w1 w2,
-        gw_accg w1 w2 -> gw_tid w1 <> gw_tid w2.
-    Proof.
-      intros. inv H. unfold gw_tid. simpl. inv H0.
-      destruct H11 as [[AA BB]_]. auto.
-    Qed.
-       
-
-    (* "(Genv.symtbl *
-   (ro_world * (Genv.symtbl * (Genv.symtbl * signature * (Genv.symtbl * (cc_cainjp_world * ext_world))))))%type" *)
-
     Inductive match_states' : global_index -> (NatMap.t (option (GS.gworld cc_compcert))) -> CMulti.state OpenC -> state OpenA -> Prop :=
       |global_match_intro : forall threadsC threadsA cur next (worldsA : NatMap.t (option (GS.ccworld cc_compcert))) worldsB worldsP gi (w0 : GS.ccworld cc_compcert) m0 main_b wPcur tm0 sp0
       (CUR_VALID: (1 <= cur < next)%nat)
@@ -351,56 +289,6 @@ Section ConcurSim.
         match_states' gi worldsP gsc gsa ->
         match_states gi gsc gsa.
 
-    Lemma foo {A: Type} (n: nat) (map : NatMap.t (option A)) (a b: A) :
-      NatMap.get n map = Some a -> NatMap.get n map = Some b -> a = b.
-    Proof.
-      intros. congruence.
-    Qed.
-
-    Lemma advance_next_tid : forall gl s s',
-        Genv.advance_next gl s = s' ->
-        Mem.tid s' = Mem.tid s.
-    Proof.
-      induction gl. intros.
-      inv H. simpl. reflexivity.
-      intros. simpl in H. apply IHgl in H. simpl in H. congruence.
-    Qed.
-
-
-    Lemma sup_incr_tid_ntid : forall s t, Mem.next_tid s = Mem.next_tid (Mem.sup_incr_tid s t).
-    Proof.
-      intros. unfold Mem.sup_incr_tid. destruct s. simpl. unfold Mem.next_tid. simpl.
-      destruct stacks; simpl. rewrite Mem.update_list_length. reflexivity.
-      rewrite Mem.update_list_length. reflexivity.
-    Qed.
-
-    Lemma advance_next_nexttid : forall gl s s',
-        Genv.advance_next gl s = s' ->
-        Mem.next_tid s' = Mem.next_tid s.
-    Proof.
-      induction gl. intros.
-      inv H. simpl. reflexivity.
-      intros. simpl in H. apply IHgl in H. simpl in H.
-      rewrite <- sup_incr_tid_ntid in H. auto.
-    Qed.
-                               
-    Lemma init_mem_tid : forall sk m, Genv.init_mem sk = Some m ->
-                                 Mem.tid (Mem.support m) = 1%nat.
-    Proof.
-      intros. unfold Genv.init_mem in H.
-      apply Genv.alloc_globals_support in H.
-      rewrite H. erewrite advance_next_tid; eauto. unfold Mem.empty.
-      reflexivity.
-    Qed.
-
-    Lemma init_mem_nexttid : forall sk m, Genv.init_mem sk = Some m ->
-                                     Mem.next_tid (Mem.support m) = 2%nat.
-    Proof.
-      intros. unfold Genv.init_mem in H.
-      apply Genv.alloc_globals_support in H.
-      rewrite H. erewrite advance_next_nexttid; eauto. unfold Mem.empty.
-      reflexivity.
-    Qed.
 
     Lemma concur_initial_states_exist :
       forall s1, Closed.initial_state ConcurC s1 ->
@@ -693,6 +581,8 @@ Section ConcurSim.
         + inv H1; unfoldC_in GET_C; rewrite NatMap.gss in GET_C; inv GET_C; eauto.
     Qed.
 
+    Hypothesis determinate_big_C : determinate_big OpenC.
+
     Lemma concur_progress : forall i s1 s2,
         match_states i s1 s2 -> Closed.safe ConcurC s1 ->
         (exists r, Closed.final_state ConcurA s2 r) \/ (exists t s2', Closed.step ConcurA (Closed.globalenv ConcurA) s2 t s2').
@@ -701,6 +591,33 @@ Section ConcurSim.
       specialize (THREADS cur CUR_VALID) as THR_CUR. 
       destruct THR_CUR as (wB & owA & wP & lsc & lsa & li & GETW & GETi & MSEw & GETC & GETA & GETWa & MS & GETWp & ACC).
       specialize (bsim_lts se tse wB MSEw valid_se) as BSIM.
+      generalize (determinate_big_C se). intro DetC.
+      inv MS.
+      - specialize (safe_concur_single _ _ Hsafe THREADS_DEFAULTC GETC). intro Hsafel.
+        exploit @GS.bsim_progress; eauto.
+        intros [[r2 F]|[[q2 X]|[t [s2' S]]]].
+        + inv BSIM. exploit bsim_match_final_states; eauto.
+          intros (s1''' & r1' & gw' & Hstar' & Hf1 & ACO & ACI & MR).
+          exploit Hsafe; eauto. eapply local_star_c; eauto.
+          admit.
+        + admit.
+        + right. do 2 eexists. econstructor; eauto.
+      - admit.
+      - admit.
+      - admit.
+      - admit.
+    Admitted.
+
+   (*
+
+
+
+      
+      intros i s1 s2 Hm Hsafe. inv Hm. inv H.
+      specialize (THREADS cur CUR_VALID) as THR_CUR. 
+      destruct THR_CUR as (wB & owA & wP & lsc & lsa & li & GETW & GETi & MSEw & GETC & GETA & GETWa & MS & GETWp & ACC).
+      specialize (bsim_lts se tse wB MSEw valid_se) as BSIM.
+      generalize (determinate_big_C se). intro DetC.
       (* start from ls2 progress, no enough info *)
       (*
         inv MS.
@@ -722,7 +639,11 @@ Section ConcurSim.
         intros [[r2 F]| [[q2 E]|[t [sa' S]]]].
         + inv BSIM. exploit bsim_match_final_states; eauto.
           intros (s1''' & r1' & gw' & Hstar' & Hf1 & ACO & ACI & MR).
-          assert (s1''' = ls /\ r1' = (cr (Vint r1) m)). admit. (*deter_big for C*)
+          assert (s1''' = ls /\ r1' = (cr (Vint r1) m)).
+          {
+            inv Hstar'. split. reflexivity. inv DetC. exploit sd_big_final_determ. apply H1. apply Hf1.
+            intro. eauto. inv DetC. exfalso. eapply sd_big_final_nostep. apply H1. apply H.
+          }
           destruct H. subst.
           left.
           destruct gw' as [p [q [wp we]]]. simpl in p, q,wp,we.
@@ -738,310 +659,65 @@ Section ConcurSim.
           rewrite H6 in H7. inv H7. reflexivity.
         + inv BSIM. exploit bsim_match_external; eauto.
           intros (wA & s1' & q1 & Hstar & X & ACI & MQ & MS & MR).
-          
-          admit.
+          inv Hstar; inv DetC; exfalso.
+          -- eapply sd_big_final_noext; eauto.
+          -- eapply sd_big_final_nostep; eauto.
+        + right. eexists. eexists. simpl. eapply step_local; eauto.
+      - inv S; unfoldC_in H. unfoldC_in H0. simpl in H0.
+        + (*local*)
+        assert (lsc = CMulti.Local OpenC ls1).
+        eapply foo; eauto. subst lsc. inv MS.
+        (* assert (wB = init_w m0 main_b tm0 sp0 INITMEM DUMMYSP).
+        eapply foo; eauto. subst wB. *)
+        specialize (safe_concur_single _ _ Hsafe THREADS_DEFAULTC GETC). intro Hsafel.
+        exploit @GS.bsim_progress; eauto.
+        intros [[r2 F]| [[q2 E]|[t' [sa' S]]]].
+        -- inv BSIM. exploit bsim_match_final_states; eauto.
+           intros (s1''' & r1' & gw' & Hstar' & Hf1 & ACO & ACI & MR).
+           exploit Hsafe. eapply local_star_c; eauto.
+           intros [[r1'2 F']| [t'2 [s1'4 S']]].
+           ++
+           inv F'. unfoldC_in H1. unfoldC_in H2. rewrite NatMap.gss in H2. inv H2. subst.
+           assert (wB = init_w m0 main_b tm0 sp0 INITMEM DUMMYSP).
+           eapply foo; eauto. subst wB. unfold CMulti.OpenLTS in H4. fold se in H4.
+           inv DetC. exploit sd_big_final_determ. apply Hf1. apply H4. intro. subst.
+           left. 
+           destruct gw' as [p [q [wp we]]]. simpl in p, q,wp,we.
+           destruct MR as [q1' [MRro [q1'' [MRwt [q2' [MRp MRe]]]]]]. destruct r2.
+           inv MRro. inv MRwt. inv MRp. inv MRe.
+           eexists. econstructor. 5: eauto. eauto. eauto.
+           assert (rs' PC = Vnullptr). eauto. generalize (H5 PC). simpl. intro.
+           rewrite H7 in H8. unfold Vnullptr in *. destr_in H8; inv H8; eauto.
+           assert (rs' RAX = Vint r1'2). subst tres.
+           unfold Conventions1.loc_result in H10. replace Archi.ptr64 with true in H10 by reflexivity.
+           simpl in H10. inv H10. reflexivity.
+           generalize (H5 RAX). simpl. intro.
+           rewrite H7 in H8. inv H8. reflexivity.
+           ++ (*kind of forward step_simulation *) admit.
+        -- inv BSIM. exploit bsim_match_external; eauto.
+           intros (wA & s1' & q1 & Hstar & X & ACI & MQ & MS & MR).
+              exploit Hsafe. eapply local_star_c; eauto.
+           intros [[r1'2 F']| [t'2 [s1'4 S']]].
+           ++
+             inv F'. unfoldC_in H1. unfoldC_in H2.
+             rewrite NatMap.gss in H2. inv H2.
+             inv DetC. exfalso. eapply sd_big_final_noext; eauto.
+           ++ (*kind of forward step_simulation *) admit.
+        -- right. do 2 eexists. econstructor; eauto.
+        +
+          assert (lsc = CMulti.Local OpenC ls).
+          eapply foo; eauto. subst lsc. inv MS.
+          specialize (safe_concur_single _ _ Hsafe THREADS_DEFAULTC GETC). intro Hsafel.
+          exploit @GS.bsim_progress; eauto.
+          intros [[r2 F]| [[q2 E]|[t [sa' S]]]].
+          -- inv BSIM. exploit bsim_match_final_states; eauto.
+             intros (s1''' & r1' & gw' & Hstar' & Hf1 & ACO & ACI & MR).
+             
         + admit.
-      - 
-          
-          
-Admitted
 
+Admitted *)
 
-
-
-
-
-
-
-          
-          (*
-   Lemma trans_pthread_create__start_routine: forall q_ptc r_ptc q_str qa_ptc wA,
-        query_is_pthread_create OpenC q_ptc r_ptc q_str ->
-        GS.match_query cc_compcert wA q_ptc qa_ptc ->
-        GS.match_senv cc_compcert wA se tse ->
-        exists gw wA' ra_ptc qa_str,
-          query_is_pthread_create_asm OpenA qa_ptc ra_ptc qa_str /\
-            gw_accg (get wA') gw /\
-            (forall w, gw_accg w (get wA) -> gw_accg w gw) /\
-            (get wA) o-> gw /\
-            gw_nexttid gw = S (gw_nexttid (get wA)) /\
-                           GS.match_reply cc_compcert (set wA gw) r_ptc ra_ptc /\
-                           GS.match_query cc_compcert wA' q_str qa_str /\
-                           GS.match_senv cc_compcert wA' se tse /\
-                           worlds_ptc_str (cainjp_w_compcert wA) (cainjp_w_compcert wA').
-   Proof.
-     intros until wA. intros H H0 MSE.
-     inv H. destruct wA as (se0 & [se0' m0'] & se1 & [se1' sig'] & se2 & w_cap & w_e).
-     destruct H0 as [q1' [Hqr [q1'' [Hqw [qa' [Hqca Hqe]]]]]].
-     inv Hqr. inv Hqw. simpl in H. destruct H0. simpl in H0. inv H0. simpl in H1.
-     inv Hqca. destruct qa_ptc as [trs ttm]. inv Hqe. destruct H2 as [PCN Hme].
-     inv Hme. clear Hm4. rename Hm3 into Hme.
-     subst tvf targs. rewrite pthread_create_locs in H5. simpl in H5.
-     inv H5. inv H17. inv H18. inv H19.
-     destruct MSE as [EQ1 [EQ2 [MSE EQ3]]].
-     inv EQ1. inv EQ2. inv EQ3. inv H2. inv H3.
-     (** prepare arguments *)
-     assert (INJPTC: j b_ptc = Some (b_ptc, 0)).
-     {
-       inv MSE. inv H17.
-       exploit mge_dom; eauto. eapply Genv.genv_symb_range. apply FINDPTC.
-       intros (b3 & INJ).
-       exploit mge_symb; eauto.
-       intro HH. apply HH in FINDPTC as FINDPTC'.
-       rewrite <- SE_eq in FINDPTC'. fold se in FINDPTC. setoid_rewrite FINDPTC in FINDPTC'.
-       inv FINDPTC'. eauto.
-     }
-     assert (PCVAL: rs PC = Vptr b_ptc Ptrofs.zero).
-     inv H6. rewrite H17 in INJPTC. inv INJPTC. reflexivity.
-     assert (INJSTR: j b_start = Some (b_start, 0)).
-     {
-       inv MSE. inv H17.
-       exploit mge_dom; eauto. eapply Genv.genv_symb_range. apply FINDSTR. eauto.
-       intros (b3 & INJ).
-       exploit mge_symb; eauto.
-       intro HH. apply HH in FINDSTR as FINDSTR'.
-       rewrite <- SE_eq in FINDSTR'. fold se in FINDSTR. setoid_rewrite FINDSTR in FINDSTR'.
-       inv FINDSTR'. eauto.
-     }
-     assert (RSIVAL: rs RSI = Vptr b_start Ptrofs.zero).
-     inv H5. rewrite H17 in INJSTR. inv INJSTR. reflexivity.
-     case (Mem.thread_create tm) as [tm' id] eqn:MEM_CREATE'.
-     exploit thread_create_inject; eauto. intros [Hm1' eqid]. subst id.
-     assert (exists b_t' ofs_t', rs RDI = Vptr b_t' ofs_t').
-     inv H11. eauto. destruct H2 as [b_t' [ofs_t' RDIVAL]].
-     assert (exists b_arg' ofs_arg', rs RDX = Vptr b_arg' ofs_arg').
-     inv H13. eauto. destruct H2 as [b_arg' [ofs_arg' RDXVAL]].
-
-     (** prepare memories *)
-     (** Here we allocate a dummy block on new thread for target memory.
-         It's address is used as the initial value of RSP on this new procedure *)
-     assert (TP1: Mem.range_prop tid (Mem.support tm')).
-     {
-       inv P1. constructor. auto. erewrite <- inject_next_tid; eauto.
-     }
-     set (tm'2 := Mem.yield tm' tid TP1).
-     case (Mem.alloc tm'2 0 0 ) as [tm'3 sp0] eqn:DUMMY.
-     assert (TP2: Mem.range_prop (Mem.tid (Mem.support tm)) (Mem.support tm'3)).
-     {
-       generalize (Mem.tid_valid (Mem.support tm)). intro.
-       constructor; eauto. lia.
-       apply Mem.support_alloc in DUMMY. rewrite DUMMY. simpl.
-       unfold Mem.next_tid, sup_incr, Mem.sup_yield. simpl.
-       rewrite Mem.update_list_length. inv MEM_CREATE'. simpl.
-       rewrite app_length. simpl. lia.
-     }
-     set (tm'4 := Mem.yield tm'3 (Mem.tid (Mem.support tm)) TP2).
-     
-     set (m1' := Mem.yield m1 tid P1).
-     assert (Hm'2 : Mem.inject j m1' tm'2).  unfold m1', tm'2.
-     eapply yield_inject. eauto.
-     assert (Hmq: Mem.inject j m1' tm'3).
-     eapply Mem.alloc_right_inject; eauto.
-     assert (Hmr: Mem.inject j m1 tm'4).
-     {
-       clear - Hm1 MEM_CREATE Hmq.
-       inv Hmq. constructor; eauto.
-       + inv mi_thread. constructor; eauto.
-         inv Hms. constructor; eauto. simpl. inv MEM_CREATE.
-         simpl. eapply inject_tid; eauto.
-       + inv mi_inj. constructor; eauto.
-     }
-          
-
-     (** similarly we need Mem.extends tm'4 ttm'4*)
-     case (Mem.thread_create ttm) as [ttm' id] eqn:MEM_CREATE'2.
-     assert (Hme1: Mem.extends tm' ttm').
-     {
-       clear - Hme MEM_CREATE' MEM_CREATE'2.
-       unfold Mem.thread_create in *. inv MEM_CREATE'.
-       inv MEM_CREATE'2. inv Hme.
-       constructor; simpl; eauto. congruence.
-       inv mext_inj. constructor; eauto.
-     }
-     assert (tid = id).
-     {
-       clear -Hme MEM_CREATE' MEM_CREATE'2.
-       unfold Mem.thread_create in *. inv MEM_CREATE'.
-       inv MEM_CREATE'2. inv Hme. rewrite mext_sup. reflexivity.
-     }
-     subst id.
-     assert (TTP1: Mem.range_prop tid (Mem.support ttm')).
-     {
-       erewrite <- Mem.mext_sup; eauto.
-     }
-     set (ttm'2 := Mem.yield ttm' tid TTP1).
-     assert (Hme2: Mem.extends tm'2 ttm'2).
-     apply yield_extends; eauto.
-     exploit Mem.alloc_extends. apply Hme2. eauto. reflexivity. reflexivity.
-     intros (ttm'3 & DUMMY2 & Hmqe).
-     assert (TTP2: Mem.range_prop (Mem.tid (Mem.support ttm)) (Mem.support ttm'3)).
-     {
-       erewrite <- Mem.mext_sup; eauto.
-       erewrite <- (Mem.mext_sup tm'3 ttm'3); eauto.
-     }
-     set (ttm'4 := Mem.yield ttm'3 (Mem.tid (Mem.support ttm)) TTP2).
-     assert (Hmre: Mem.extends tm'4 ttm'4).
-     apply yield_extends; eauto. inv Hme. congruence.
-     
-     set (rs_q := rs # PC <- (rs RSI) # RDI <- (rs RDX) # RSP <- (Vptr sp0 Ptrofs.zero)).
-     set (rs_r := rs # PC <- (rs RA) # RAX <- (Vint Int.one)).
-     set (trs_q := trs # PC <- (trs RSI) # RDI <- (trs RDX) # RSP <- (Vptr sp0 Ptrofs.zero)).
-     set (trs_r := trs # PC <- (trs RA) # RAX <- (Vint Int.one)).
-     rename H0 into RSLD. simpl in RSLD.
-     eapply lessdef_trans in PCVAL as PCVAL'; eauto.
-     eapply lessdef_trans in RSIVAL as RSIVAL'; eauto.
-     eapply lessdef_trans in RDIVAL as RDIVAL'; eauto.
-     eapply lessdef_trans in RDXVAL as RDXVAL'; eauto.
-     inv H.
-     exists (tt, (tt, (injpw j m1 tm'4 Hmr, extw tm'4 ttm'4 Hmre))).
-     exists (se, ((row se m1'), (se, (se, start_routine_sig, (tse,((cajw (injpw j m1' tm'3 Hmq) start_routine_sig rs_q) , extw tm'3 ttm'3 Hmqe))) ))).
-     exists (trs_r, ttm'4). exists (trs_q, ttm'3).
-     assert (UNC23: Mem.unchanged_on (fun _ _ => True) tm'2 tm'3). eapply Mem.alloc_unchanged_on. eauto.
-     assert (UNC23': Mem.unchanged_on (fun _ _ => True) ttm'2 ttm'3). eapply Mem.alloc_unchanged_on. eauto.
-     apply Mem.support_alloc in DUMMY as HSUP.
-     apply Mem.support_alloc in DUMMY2 as HSUP2. simpl.
-     assert (ROACCR1 : ro_acc m m1). eapply ro_acc_thread_create; eauto.
-     assert (ROACCQ1: ro_acc m m1'). eapply ro_acc_trans. eauto. eapply ro_acc_yield; eauto. reflexivity.
-     assert (ROACCQ2: ro_acc tm tm'3).
-     eapply ro_acc_trans. eapply ro_acc_thread_create; eauto.
-     eapply ro_acc_trans. eapply ro_acc_yield. 
-     instantiate (1:= tm'2). reflexivity. eapply ro_acc_alloc; eauto.
-     assert (ROACCR2: ro_acc tm tm'4). eapply ro_acc_trans. eauto. eapply ro_acc_yield; eauto. reflexivity.
-     assert (ROACCQ3: ro_acc ttm ttm'3).
-      eapply ro_acc_trans. eapply ro_acc_thread_create; eauto.
-     eapply ro_acc_trans. eapply ro_acc_yield. 
-     instantiate (1:= ttm'2). reflexivity. eapply ro_acc_alloc; eauto.
-     assert (ROACCR3: ro_acc ttm ttm'4). eapply ro_acc_trans. eauto. eapply ro_acc_yield; eauto. reflexivity.
-     assert (SINC1: Mem.sup_include (Mem.support tm) (Mem.support tm'4)).
-     { inv ROACCR2. eauto. }
-     assert (SINC2: Mem.sup_include (Mem.support ttm) (Mem.support ttm'4)).
-     { inv ROACCR3. eauto. } 
-     repeat apply conj.
-     - fold se in FINDPTC. rewrite SE_eq in FINDPTC.
-       fold se in FINDSTR. rewrite SE_eq in FINDSTR.
-       econstructor.
-       eapply FINDPTC. eapply FINDSTR. eauto. eauto. eauto. eauto. reflexivity.
-       unfold trs_q. instantiate (1:= sp0). rewrite RDXVAL'.
-       rewrite RSIVAL'. reflexivity.
-       eauto. eauto.
-       instantiate (1:= TTP1). fold ttm'2. eauto. reflexivity.
-     - (** accg *)
-       simpl. econstructor.
-       econstructor; eauto; try red; intros; try congruence; eauto.
-       split. split; eauto. inv MEM_CREATE. simpl. generalize (Mem.tid_valid (Mem.support m)). intro. unfold Mem.next_tid. lia.
-       inv MEM_CREATE. constructor; eauto. simpl. red. intros. eauto with mem.
-       intros. reflexivity.
-       split. split; eauto.
-       simpl. erewrite Mem.support_alloc; eauto. simpl. inv MEM_CREATE'. simpl.
-       generalize (Mem.tid_valid (Mem.support tm)). intro. unfold Mem.next_tid. lia.
-       constructor; eauto. simpl. red. intros. eauto with mem. intros. reflexivity.
-       {
-         unfold tm'4, ttm'4.
-         econstructor; simpl.
-         erewrite Mem.support_alloc; eauto. simpl. inv MEM_CREATE'.
-         generalize (Mem.tid_valid (Mem.support tm)). intro. unfold Mem.next_tid. lia.
-         erewrite Mem.support_alloc; eauto. simpl. inv MEM_CREATE'2.
-         generalize (Mem.tid_valid (Mem.support ttm)). intro. unfold Mem.next_tid. lia.
-         red. intros. eauto with mem. red. intros. eauto with mem.
-         red. intros. eauto with mem. red. intros. eauto with mem.
-       }
-     - intros. inv H. inv MEM_CREATE. inv MEM_CREATE'. constructor.
-       unfold injp_gw_compcert.
-       simpl. inv H17.
-       assert (ROACC: ro_acc m2 tm'4). eapply ro_acc_trans. 2: eauto.
-       destruct H28 as [_ [A _]]. constructor; eauto.
-       econstructor; eauto.
-       + inv ROACC. eauto.
-       + inv ROACC. eauto.
-       + destruct H27 as [[A B] C]. constructor; simpl. split. unfold Mem.next_tid, Mem.sup_create in *. simpl. rewrite app_length. simpl. lia.
-         lia. inv C. constructor; simpl. eapply Mem.sup_include_trans. eauto. red. intros. rewrite <- Mem.sup_create_in. auto.
-         intros. etransitivity. eauto. reflexivity. intros. etransitivity. reflexivity. eauto.
-       + destruct H28 as [[A B] C]. constructor; simpl. split. etransitivity. eauto.
-         unfold Mem.next_tid, Mem.sup_yield. simpl.
-         rewrite HSUP. simpl. rewrite Mem.update_list_length. rewrite app_length. simpl. lia. lia.
-         inv C. constructor; simpl. eapply Mem.sup_include_trans. eauto. red. intros. rewrite <- Mem.sup_yield_in.
-         rewrite HSUP. apply Mem.sup_incr_in2. simpl. rewrite <- Mem.sup_yield_in, <- Mem.sup_create_in. eauto.
-         intros. etransitivity. eauto. transitivity (Mem.perm tm'2 b ofs k p). reflexivity.
-         transitivity (Mem.perm tm'3 b ofs k p). 2: reflexivity. inv UNC23. apply unchanged_on_perm0; eauto.
-         red. simpl. rewrite <- Mem.sup_yield_in, <- Mem.sup_create_in. eauto.
-         intros. inv UNC23. rewrite unchanged_on_contents0; eauto. apply unchanged_on_perm in H0; eauto with mem.
-       + inv H21. inv ROACCR2. inv ROACCR3.
-         constructor; simpl. eauto. eauto.
-         eapply Mem.sup_include_trans; eauto.
-         eapply Mem.sup_include_trans; eauto.
-         eapply max_perm_decrease_trans. apply MPD1. eauto. eauto.
-         eapply max_perm_decrease_trans. apply MPD2. eauto. eauto.
-     - auto.
-     - auto.
-     - simpl. inv MEM_CREATE. inv MEM_CREATE'.
-       constructor; simpl; eauto; try red; intros; simpl in *; try congruence; eauto.
-       assert (Mem.loadbytes tm'3 b ofs n = Some bytes). eauto.
-       erewrite Mem.loadbytes_unchanged_on_1 in H17. 2: eauto. eauto.
-       red. simpl. rewrite <- Mem.sup_yield_in, <- Mem.sup_create_in. eauto.
-       intros. simpl. reflexivity.
-       assert (Mem.perm tm'3 b ofs Max p). eauto.
-       exploit Mem.perm_unchanged_on_2; eauto. reflexivity.
-       red. simpl. rewrite <- Mem.sup_yield_in, <- Mem.sup_create_in. eauto.
-       split. split; simpl; eauto. rewrite app_length. simpl. lia. constructor; simpl; eauto. 
-       red. intros. rewrite <- Mem.sup_create_in. auto. intros. reflexivity.
-       split. split; simpl; eauto. rewrite HSUP. simpl. rewrite Mem.update_list_length. rewrite app_length. simpl. lia.
-       constructor; eauto.
-       intros. unfold tm'4. transitivity (Mem.perm tm'2 b ofs k p). reflexivity.
-       transitivity (Mem.perm tm'3 b ofs k p). 2: reflexivity.
-       inv UNC23. apply unchanged_on_perm; eauto. red. simpl. rewrite <- Mem.sup_yield_in, <- Mem.sup_create_in. eauto.
-       intros. transitivity (  Maps.ZMap.get ofs (NMap.get (Maps.ZMap.t memval) b (Mem.mem_contents tm'2))).
-       2: reflexivity.
-       inv UNC23. apply unchanged_on_contents; eauto.
-     - simpl. constructor; eauto. inv ROACCR2. eauto. inv ROACCR3. eauto.
-     - unfold gw_nexttid. simpl. inv MEM_CREATE. simpl. unfold Mem.sup_create. unfold Mem.next_tid.
-       simpl. rewrite app_length. simpl. lia.
-     - econstructor; eauto.
-       split. econstructor; eauto. constructor. eauto.
-       eexists. split. econstructor; eauto. 
-       unfold pthread_create_sig. simpl. auto.
-       exists (rs_r, tm'4). split. econstructor; eauto.
-       unfold pthread_create_sig. simpl.
-       unfold Conventions1.loc_result. replace Archi.ptr64 with true. simpl.
-       unfold rs_r. rewrite Pregmap.gss. constructor. eauto.
-       intros. unfold rs_r. rewrite !Pregmap.gso; eauto.
-       destruct r; simpl in H1; simpl; congruence.
-       destruct r; simpl in H; simpl; congruence.
-       constructor; simpl; eauto.
-       intros. unfold rs_r. unfold trs_r.
-       setoid_rewrite Pregmap.gsspec. destr. constructor.
-       setoid_rewrite Pregmap.gsspec. destr. eauto. eauto. constructor.
-     - eexists. split. econstructor; eauto. econstructor.
-       eapply ro_acc_sound; eauto.
-       eexists. split. econstructor; eauto. simpl. intuition auto.
-       exists (rs_q, tm'3). split.
-       econstructor; eauto. rewrite start_routine_loc. simpl.
-       constructor. unfold rs_q. rewrite Pregmap.gso; try congruence.
-       rewrite Pregmap.gss. eauto.
-       constructor. unfold Conventions.size_arguments.
-       rewrite start_routine_loc. simpl. intros. inv H. extlia.
-       unfold rs_q. rewrite Pregmap.gss. constructor.
-       eapply Hvalid; eauto. eapply Hlocal; eauto.
-       econstructor. unfold Conventions.tailcall_possible, Conventions.size_arguments.
-       rewrite start_routine_loc. simpl. reflexivity. congruence.
-       constructor; eauto. simpl. unfold rs_q, trs_q. intros.
-       setoid_rewrite Pregmap.gsspec. destr. apply val_inject_id. constructor.
-       setoid_rewrite Pregmap.gsspec. destr. eauto.
-       setoid_rewrite Pregmap.gsspec. destr. eauto. eauto.
-       split. unfold rs_q. rewrite Pregmap.gso; try congruence.
-       rewrite Pregmap.gso; try congruence. rewrite Pregmap.gss. congruence.
-       constructor.
-     - constructor. reflexivity.
-     - constructor. reflexivity.
-     - inv MSE. constructor; eauto. inv ROACCQ1. eapply Mem.sup_include_trans; eauto.
-     - reflexivity.
-     - econstructor; eauto. reflexivity.
-     - congruence.
-     - congruence.
-     - congruence.
-   Qed.
-*)
-    
-
+   
    Lemma substep_switch_out : forall i s1 s2 s2' target m',
        match_states i s1 s2 ->
        AsmMulti.switch_out OpenA s2 s2' target m' ->
@@ -1067,305 +743,7 @@ Admitted
        clear bsim_simulation bsim_match_initial_states
          bsim_match_final_states.
    Admitted.
-   (*
-       exploit bsim_match_external; eauto.
-       red.
-       intros (wA & [rs_q tm_q] & HX & GW_ACC & MQ & MS & MR).
-       assert (wP = wPcur). congruence. subst wP.
-       destruct wA as (se0 & [se0' m0'] & se1 & [se1' sig'] & se2 & w_cap & w_e).
-       destruct MQ as [q1' [Hqr [q1'' [Hqw [qa' [Hqca Hqe]]]]]].
-       inv Hqr. inv Hqw. simpl in H. destruct H1. simpl in H1. inv H1. simpl in H.
-       inv Hqca. inv Hqe. destruct H13 as [PCN Hme].
-       inv Hme. clear Hm3. rename Hm2 into Hme.
-       destruct MS as [EQ1 [EQ2 [MSE EQ3]]]. inv EQ1. inv EQ2. inv EQ3.
-       inv H13. inv H14.
-       rename tm_q into ttm_q. rename rs_q into rrs_q. rename rs into rs_q. rename tm into tm_q.
-       assert (tp : Mem.range_prop target (Mem.support(tm_q))).
-       { red. red in p. simpl in p. inversion Hm.
-         inv mi_thread. inv Hms.
-         setoid_rewrite <- H13. auto. }
-       set (tm' := Mem.yield tm_q target tp).
-       simpl.
-       set (wAca := {| cajw_injp := injpw j m tm_q Hm; cajw_sg := sg; cajw_rs := rs_q |}).
-       set (m' := Mem.yield m target p).
-       assert (Hm' : Mem.inject j m' tm').
-       exploit yield_inject; eauto.
-       assert (ttp : Mem.range_prop target (Mem.support (ttm_q))).
-       { erewrite <- Mem.mext_sup; eauto. }
-       set (ttm' := Mem.yield ttm_q target ttp).
-       assert (Hme' : Mem.extends tm' ttm').
-       eapply yield_extends; eauto.
-       inv H.
-       eexists. exists tm', ttm'.
-       set (wpj := injpw j m tm_q Hm).
-       set (wpj' := injpw j m' tm' Hm').
-       set (wp:= (tt,(tt,(wpj, extw tm_q ttm_q Hm1)))).
-       set (wp' := (tt,(tt,(wpj', extw tm' ttm' Hme')))).
-       (*exists (se, ((row se m1'), (se, (se, start_routine_sig, (tse,((cajw (injpw j m1' tm'3 Hmq) start_routine_sig rs_q) , extw tm'3 ttm'3 Hmqe))) ))). *)
-       set (wA := (se,(row se m,(se,(se, sg, (tse,(wAca,extw tm_q ttm_q Hm1))))))).
-       exists (NatMap.set cur (Some wp) worldsP), wp, j, Hme', Hm'.
-       repeat apply conj.
-       + (*step*)
-         eapply switch_out_yield. eauto. eauto.
-         { inv Q_YIE. inv MSE.
-           econstructor. fold tse. rewrite <- SE_eq. eauto.
-           subst tvf. inv H3.
-           rewrite <- SE_eq in H16.
-           exploit match_senv_id. eauto. apply H17. eauto. intros [X Y].
-           subst b delta. symmetry in H15. eapply lessdef_trans in H15; eauto.
-           simpl. simpl in H19. erewrite <- Mem.mext_sup. 2: eauto.
-           inv Hm3. inv mi_thread. inv Hms. unfold Mem.next_tid. auto.
-         }
-         reflexivity.
-         reflexivity.
-       + (*match_states*)
-         apply gw_acci_nexttid in GW_ACC as NTID. apply gw_acci_tid in GW_ACC as TID.
-         econstructor. 8:{ rewrite NatMap.gss. reflexivity. }
-         all : simpl; eauto.
-         -- simpl. intros. destruct (Nat.eq_dec 1 cur).
-            subst. rewrite NatMap.gss. congruence.
-            rewrite NatMap.gso; eauto.
-         -- destruct CUR_INJP_TID as [X Y]. split.
-            rewrite <- X in TID. simpl in TID.
-            unfold gw_tid in TID. simpl in TID. unfold gw_tid. simpl. congruence.
-            rewrite <- Y in NTID. simpl in NTID.
-            unfold gw_nexttid in NTID. simpl in NTID. unfold gw_nexttid. simpl. congruence.
-         -- destruct CUR_INJP_TID.  simpl in *.
-            intros. destruct (Nat.eq_dec n cur). subst.
-            rewrite NatMap.gss in H15. inv H15.
-            split. eauto. lia. 
-            rewrite NatMap.gso in H15.
-            exploit FIND_TID; eauto. eauto.
-         -- intros.
-            instantiate (1:= NatMap.set cur (Some wA) worldsA).
-            destruct (Nat.eq_dec n cur).
-            ++ subst n.
-               exists wB, (Some wA), wp. eexists. eexists. exists li.
-               repeat apply conj; eauto. rewrite NatMap.gss. reflexivity.
-               rewrite NatMap.gss. reflexivity. rewrite NatMap.gss. reflexivity.
-               simpl. simpl in wp'. assert (HRS: rs_q = cajw_rs wAca).  reflexivity.
-               eapply match_returny; eauto.
-               unfold wA. econstructor; eauto.
-               inversion Q_YIE. subst m1 args sg vf next0. eauto.
-               red. intros. apply val_inject_id. eauto. simpl in MR.
-               rewrite NatMap.gss. eauto. simpl. congruence.
-            ++ (* clear - THREADS H3 OTHERi n0. *)
-               destruct (THREADS n H) as (wn & owan & wnp & lscn & lsan & lin & A & B & C & D & E & F & G & I & J).
-               exists wn, owan, wnp, lscn,lsan,lin. repeat apply conj; eauto.
-               rewrite NatMap.gso. simpl. eauto. lia.
-               rewrite NatMap.gso. simpl. eauto. lia.
-               rewrite NatMap.gso. simpl. eauto. lia.
-               rewrite NatMap.gso. simpl. eauto. lia.
-               simpl. intros. specialize (J H13).
-               eapply gw_accg_acci_accg; eauto. constructor.
-       + intros. simpl. unfold CMulti.get_cur_thread, CMulti.update_cur_thread. simpl.
-         unfold CMulti.get_thread, CMulti.update_thread. simpl. rewrite NatMap.gss. congruence.
-       + rewrite NatMap.gss. eauto.
-       + econstructor; eauto. econstructor; eauto.
-         reflexivity. reflexivity. econstructor; eauto. reflexivity. reflexivity.
-       + eauto.
-     - (** join *)
-       specialize (THREADS cur CUR_VALID) as THR_CUR.
-       destruct THR_CUR as (wB & owA & wP & lsc & lsa & li & GETW & GETi & MSEw & GETC & GETA & GETWa & MS & GETWp & ACC).
-       assert (lsc = CMulti.Local OpenC ls).
-       eapply foo; eauto. subst lsc. inv MS.
-       specialize (fsim_lts se tse wB MSEw valid_se) as FSIM.
-       inversion FSIM.
-       clear fsim_simulation fsim_match_initial_states
-            fsim_match_final_states.
-       exploit fsim_match_external; eauto. intros (wA & [rs_q tm_q] & HX & GW_ACC & MQ & MS & MR).
-       assert (wP = wPcur). congruence. subst wP.
-       destruct wA as (se0 & [se0' m0'] & se1 & [se1' sig'] & se2 & w_cap & w_e).
-       destruct MQ as [q1' [Hqr [q1'' [Hqw [qa' [Hqca Hqe]]]]]].
-       inv Hqr. inv Hqw. simpl in H. destruct H1. simpl in H1. inv H1. simpl in H.
-       inv Hqca. inv Hqe. destruct H13 as [PCN Hme].
-       inv Hme. clear Hm3. rename Hm2 into Hme.
-       destruct MS as [EQ1 [EQ2 [MSE EQ3]]]. inv EQ1. inv EQ2. inv EQ3.
-       inv H13. inv H14. inv MSE.
-       rename tm_q into ttm_q. rename rs_q into rrs_q. rename rs into rs_q. rename tm into tm_q.
-       inv Q_JOIN.
-       subst targs tvf.
-       setoid_rewrite pthread_join_locs in H1. simpl in H1.
-       inv H1. inv H21. inv H22.
-       assert (HPC: rs_q PC = Vptr b_ptj Ptrofs.zero).
-       inv H3. rewrite <- SE_eq in H16. exploit match_senv_id; eauto. intros [X Y].
-       subst b2 delta. reflexivity.
-       assert (HRDI: rs_q RDI = Vint i0). inv H17. eauto.
-       assert (HRSI: exists b_vptr' ofs_vptr', rs_q RSI = Vptr b_vptr' ofs_vptr').
-       inv H15. eauto. destruct HRSI as [b_vptr' [ofs_vptr' HRSI]].
-       eapply lessdef_trans in HPC as HPC'; eauto.
-       eapply lessdef_trans in HRDI as HRDI'; eauto.
-       eapply lessdef_trans in HRSI as HRSI'; eauto.
-       
-       assert (tp : Mem.range_prop target (Mem.support(tm_q))).
-       red. red in p. simpl in p. inversion Hm.
-       inv mi_thread. inv Hms. setoid_rewrite <- H1. auto.
-       set (tm' := Mem.yield tm_q target tp).
-       set (wAca := {| cajw_injp := injpw j m tm_q Hm; cajw_sg := pthread_join_sig; cajw_rs := rs_q |}).
-       set (m' := Mem.yield m target p).
-       assert (Hm': Mem.inject j m' tm'). eapply yield_inject; eauto.
-       assert (ttp: Mem.range_prop target (Mem.support (ttm_q))).
-       erewrite <- Mem.mext_sup; eauto.
-       set (ttm' := Mem.yield ttm_q target ttp).
-       assert (Hme' : Mem.extends tm' ttm'). eapply yield_extends; eauto.
-       set (wpj := injpw j m tm_q Hm).
-       set (wpj' := injpw j m' tm' Hm').
-       set (wp:= (tt,(tt,(wpj, extw tm_q ttm_q Hm1)))).
-       set (wp' := (tt,(tt,(wpj', extw tm' ttm' Hme')))).
-       inv H.
-       set (wA := (se,(row se m,(se,(se, pthread_join_sig, (tse,(wAca,extw tm_q ttm_q Hm1))))))).
-       eexists. exists tm', ttm'. exists (NatMap.set cur (Some wp) worldsP). exists wp,j,Hme', Hm'.
-       repeat apply conj; try rewrite NatMap.gss; eauto.
-       + (*step*)
-         eapply switch_out_join. eauto. eauto.
-         econstructor; eauto.
-         fold tse. rewrite <- SE_eq. eauto. eauto. reflexivity. reflexivity.
-       + (*match_states*)
-         apply gw_acci_nexttid in GW_ACC as NTID. apply gw_acci_tid in GW_ACC as TID.
-         simpl in *.
-         econstructor. 8:{ rewrite NatMap.gss. reflexivity. }
-         all : simpl; eauto.
-         -- simpl. intros. destruct (Nat.eq_dec 1 cur).
-            subst. rewrite NatMap.gss. congruence.
-            rewrite NatMap.gso; eauto.
-         -- destruct CUR_INJP_TID as [X Y]. split.
-            rewrite X. rewrite <- TID. reflexivity.
-            rewrite Y. rewrite <- NTID. reflexivity.
-         -- destruct CUR_INJP_TID.
-            intros. destruct (Nat.eq_dec n cur). subst.
-            rewrite NatMap.gss in H14. inv H14.
-            split. eauto. lia. 
-            rewrite NatMap.gso in H14.
-            exploit FIND_TID; eauto. eauto.
-         -- intros.
-            instantiate (1:= NatMap.set cur (Some wA) worldsA).
-            destruct (Nat.eq_dec n cur).
-            ++ subst n.
-               exists wB, (Some wA), wp. eexists. eexists. exists li.
-               repeat apply conj; eauto. rewrite NatMap.gss. reflexivity.
-               rewrite NatMap.gss. reflexivity. rewrite NatMap.gss. reflexivity.
-               simpl. simpl in wp.
-               eapply match_returnj; eauto.
-               red. intros. eapply val_inject_id; eauto.
-               simpl. rewrite HRSI'. rewrite <- HRSI. eauto.
-               unfold wA. constructor.
-               rewrite NatMap.gss. eauto. simpl. congruence.
-            ++ (* clear - THREADS H3 OTHERi n0. *)
-               destruct (THREADS n H) as (wn & owan & wnp & lscn & lsan & lin & A & B & C & D & E & F & G & I & J).
-               exists wn, owan, wnp, lscn,lsan,lin. repeat apply conj; eauto.
-               rewrite NatMap.gso. simpl. eauto. lia.
-               rewrite NatMap.gso. simpl. eauto. lia.
-               rewrite NatMap.gso. simpl. eauto. lia.
-               rewrite NatMap.gso. simpl. eauto. lia.
-               simpl. intros. specialize (J H1).
-               eapply gw_accg_acci_accg; eauto. constructor.
-       +  intros. simpl. unfold CMulti.get_cur_thread, CMulti.update_cur_thread. simpl.
-         unfold CMulti.get_thread, CMulti.update_thread. simpl. rewrite NatMap.gss. congruence.
-       + econstructor; eauto; econstructor; eauto; reflexivity.
-       + congruence.
-       + congruence.
-     - (** final *)
-       specialize (THREADS cur CUR_VALID) as THR_CUR.
-       destruct THR_CUR as (wB & owA & wP & lsc & lsa & li & GETW & GETi & MSEw & GETC & GETA & GETWa & MS & GETWp & ACC).
-       assert (lsc = CMulti.Local OpenC ls).
-       eapply foo; eauto. subst lsc. inv MS.
-       specialize (fsim_lts se tse wB MSEw valid_se) as FSIM.
-       inversion FSIM.
-       clear fsim_simulation fsim_match_initial_states fsim_match_external.
-       exploit fsim_match_final_states; eauto.
-       intros ([rs_r tm_r] & gw' & FINAL' & GW_ACC_IF & GW_ACC_BIG & MR).
-       assert (wP = wPcur). congruence. subst wP.
-       destruct wB as (se0 & [se0' m0'] & se1 & [se1' sig'] & se2 & w_cap & w_e).
-       destruct gw' as [pp [qq [gwp' gwe']]]. simpl in MR.
-       destruct MR as [r1' [Hrr [r1'' [Hrw [qa' [Hrca Hre]]]]]].
-       assert (sig' = start_routine_sig).
-       {
-         exploit SUB_THREAD_SIG; eauto. intros [A B].
-         eauto.
-       }
-       assert (SIG2: cajw_sg w_cap = start_routine_sig).
-       { exploit SUB_THREAD_SIG; eauto. intros [A B]. eauto. }
-       subst sig'.
-       inv Hrr. inv Hrw. simpl in H. inv H. simpl in H1.
-       inv Hrca. inv Hre. inv H4. clear Hm2. rename Hm1 into Hme.
-       destruct MSEw as [EQ1 [EQ2 [MSE EQ3]]]. inv EQ1. inv EQ2. inv EQ3.
-       inv H4. inv H8. inv MSE.
-       rename tm_r into ttm_r. rename rs_r into rrs_r.
-       rename rs' into rs_r. rename tm' into tm_r.
-       simpl in H2. simpl in gwp'.
-       
-       assert (tp : Mem.range_prop target (Mem.support(tm_r))).
-       red. red in p. simpl in p. inversion Hm'0.
-       inv mi_thread. inv Hms. setoid_rewrite <- H12. auto.
-       set (tm' := Mem.yield tm_r target tp).
-       set (m' := Mem.yield gmem target p).
-       rename j' into j. rename Hme into Hme_r. rename Hm into Hme. rename Hm' into Hm.
-       assert (Hmj' : Mem.inject j m' tm'). eapply yield_inject; eauto.
-
-
-       assert (ttp: Mem.range_prop target (Mem.support (ttm_r))).
-       erewrite <- Mem.mext_sup; eauto.
-       set (ttm' := Mem.yield ttm_r target ttp).
-       assert (Hme' : Mem.extends tm' ttm'). eapply yield_extends; eauto.
-
-       set (wpj := injpw j gmem tm_r Hm).
-       set (wpj' := injpw j m' tm' Hmj').
-       set (wp:= (tt,(tt,(wpj, extw tm_r ttm_r Hme_r)))).
-       set (wp' := (tt,(tt,(wpj', extw tm' ttm' Hme')))).
-       (* set (wA := (se,(row se m0',(se,(se, pthread_join_sig, (tse,(wAca,extw tm_q ttm_q Hm1))))))).
-       set (wp' := injpw j m' tm' Hmj'). *)
-       set (gw' := (tt,(tt,(gwp', extw tm_r ttm_r Hme)))).
-       set (wB := (se,( row se m0',(se,(se, start_routine_sig ,(tse,(w_cap,w_e))))))).
-       eexists. exists tm', ttm'. exists (NatMap.set cur (Some gw') worldsP). exists gw',j, Hme', Hmj'.
-       repeat apply conj; try rewrite NatMap.gss; eauto.
-       + (*step*)
-         eapply switch_out_final. eauto. eauto. eauto. reflexivity. reflexivity.
-         econstructor; eauto.
-       + (*match_states*)
-         simpl in *.
-         econstructor.
-         8:{  rewrite NatMap.gss. reflexivity. }
-         all: simpl; eauto.
-         -- intros. destruct (Nat.eq_dec 1 cur).
-            subst. rewrite NatMap.gss. congruence.
-            rewrite NatMap.gso. eauto. eauto.
-         -- destruct   CUR_INJP_TID as [X Y]. split.
-            apply gw_acci_tid in GW_ACC_BIG. rewrite X. rewrite <- GW_ACC_BIG. reflexivity.
-            apply gw_acci_nexttid in GW_ACC_BIG. rewrite Y. rewrite <- GW_ACC_BIG. reflexivity.
-         -- destruct   CUR_INJP_TID as [X Y].
-            intros. destruct (Nat.eq_dec n cur). subst. rewrite NatMap.gss in H12. inv H12.
-            split. apply gw_acci_tid in GW_ACC_BIG. auto. lia.
-            rewrite NatMap.gso in H12. eauto. eauto.
-         -- intros.
-            instantiate (1:= worldsA). 
-            destruct (Nat.eq_dec n cur).
-            ++ subst n.
-               exists wB, None. eexists. eexists. eexists. exists li.
-               repeat apply conj; eauto. constructor. reflexivity.
-               constructor. reflexivity. destruct w_cap. rewrite <- H4. constructor; eauto.
-               rewrite NatMap.gss. reflexivity.
-               rewrite NatMap.gss. reflexivity.
-               eapply match_final_sub.
-               instantiate (1:= gw').
-               subst tres. unfold injp_gw_compcert. simpl. destruct w_cap.
-               inv H. simpl. simpl in SIG2. subst.
-               eapply Mem.val_inject_lessdef_compose. eauto. apply val_inject_id.
-               apply H2.
-               rewrite NatMap.gss. eauto. intros. extlia.
-            ++ (* clear - THREADS H3 OTHERi n0. *)
-               destruct (THREADS n H12) as (wn & owan & wnp & lscn & lsan & lin & A & B & C & D & E & F & G & I & J).
-               exists wn, owan, wnp, lscn,lsan,lin. repeat apply conj; eauto.
-               rewrite NatMap.gso. simpl. eauto. lia.
-               rewrite NatMap.gso. simpl. eauto. lia.
-               rewrite NatMap.gso. simpl. eauto. lia.
-               intros. specialize (J H13). eapply gw_accg_acci_accg; eauto.
-               unfold gw'. destruct w_cap. simpl in H. inv H. constructor.
-       + intros. simpl. unfold CMulti.get_cur_thread, CMulti.update_cur_thread. simpl.
-         unfold CMulti.get_thread, CMulti.update_thread. simpl. rewrite NatMap.gss. congruence.
-       + unfold gw'. destruct w_cap. simpl in H. inv H. constructor; eauto; econstructor; eauto; reflexivity.
-   Qed.
-    *)
-   
+  
    Lemma substep_switch_in : forall i s1' s2' s1'' target m' tm' ttm' f Hmj' Hme' worldsP wpc,
        (* sth more about gtmem'*)
        let cur := CMulti.cur_tid OpenC s1' in
@@ -1379,599 +757,34 @@ Admitted
              match_states i' s1'' s2''.
    Proof.
    Admitted.
-   (*
-     intros until wpc. intros cur MS' GETwpc NOTINIT ACCY TID_TARGET SWITCH.
-     assert (RANGE: (1 <= target < CMulti.next_tid OpenC s1')%nat).
-     {
-       inv ACCY. simpl. inv MS'. simpl. simpl in cur. subst cur.
-       assert ((tt,(tt,(injpw f m1 m2 Hmj,extw m2 m3 Hme0))) = wPcur).
-       congruence.
-       destruct CUR_INJP_TID. rewrite H1. rewrite <- H. simpl. unfold gw_nexttid. simpl.
-       inv H2. eauto.
-     }
-     inv MS'. set (target := Mem.tid (Mem.support m')).
-     simpl in cur. subst cur. rename cur0 into cur.
-     destruct (Nat.eq_dec cur target).
-     - (*switch to self*)
-       simpl in RANGE.
-       specialize (THREADS target RANGE) as THR_TAR.
-       destruct THR_TAR as (wB & owA & wP & lsc & lsa & li & GETW & GETi & MSEw & GETC & GETA & GETWa & MS & GETWp & ACC).
-       assert (wpc = wP). congruence. subst wpc.
-       inv SWITCH.
-       + (*yield*)
-         assert (lsc = CMulti.Returny OpenC ls1).
-         eapply foo; eauto. subst lsc. inv MS. 
-         assert (get wA = wPcur). clear -GETWp CUR_GWORLD.
-         rewrite CUR_GWORLD in GETWp. inv GETWp. reflexivity.
-         subst wPcur.
-         apply FIND_TID in GETWp as X. destruct X as [HwaTid RNGtarget].
-         destruct wA as (se0 & [se0' m0'] & se1 & [se1' sig'] & se2 & wAca & wAe).
-         simpl in GETwpc, ACCY, ACC, GETWp, HwaTid, RSLD.
-         inv ACCY.
-         assert (ACCEJ: injp_acce (get_injp wAca) (injpw f m' tm' Hmj')).
-         { eapply injp_acc_yield_acce. eauto. rewrite <- H. inv H3.
-           econstructor; eauto. eauto. }
-         assert (ACCEE: ext_acce (extw m2 m3 Hme0) (extw tm' ttm' Hme')).
-         {
-           assert (BASE:injp_tid (get_injp wAca) = injp_tid (injpw f m' tm' Hmj')).
-           eauto. eapply ext_acc_yield_acce; eauto. inv H8. econstructor; eauto.
-           simpl. rewrite <- H in BASE. simpl in BASE.
-           erewrite <- inject_tid. 2: eauto. rewrite BASE.
-           erewrite inject_tid; eauto.
-         }
-         set (qc := cr Vundef m'). rename rs into trs.
-         set (rs := cajw_rs wAca).
-         set (rs' := Pregmap.set PC (rs RA) rs).
-         set (trs' := Pregmap.set PC (trs RA) trs).
-         set (r_a := (rs', tm')).
-         set (tr_a := (trs', ttm')).
-         exploit M_REPLIES; eauto. 
-         instantiate (1:= (tt, (tt, (injpw f m' tm' Hmj', extw tm' ttm' Hme')))).
-         repeat apply conj; simpl; eauto.
-         instantiate (1:= tr_a). unfold tr_a.
-         { 
-           eexists. split. instantiate (1:= cr Vundef m').
-           econstructor; eauto. constructor.
-           inv WT_WA. simpl in ACCEJ. inv ACCEJ. constructor; eauto. destruct H14 as [_ [A _]]. auto.
-           eexists. split. econstructor; eauto. constructor.
-           exists r_a. split. unfold r_a. simpl. destruct wAca. simpl. destruct cajw_injp.
-           econstructor; eauto.
-           intros. unfold rs'.
-           destruct r; simpl in H; inv H; repeat rewrite Pregmap.gso;
-             simpl; try congruence; try reflexivity.
-           econstructor; simpl; eauto. unfold rs_w_compcert in RSLD. simpl in RSLD.
-           unfold rs', trs'. intros. setoid_rewrite Pregmap.gsspec.
-           destr; apply val_inject_id; eauto. constructor.
-         } 
-           intros (li' & sa' & AFT_E' & MLS').
-           specialize (get_nth_set (target-1) i li li' GETi) as SETi.
-           destruct SETi as (i' & SETi & Newi & OTHERi).
-         eexists. exists i'. split.
-         (*switch_in*)
-         econstructor; eauto.
-         (*match*)
-         set (wpj' := injpw f m' tm' Hmj').
-         set (wp' := (tt,(tt,(wpj', extw tm' ttm' Hme')))).
-         econstructor. instantiate (1:= NatMap.set target (Some wp') worldsP).
-         econstructor; simpl. 8:{  rewrite NatMap.gss. reflexivity. }
-         all: eauto.
-         -- erewrite set_nth_error_length; eauto.
-         -- intros. fold target. destruct (Nat.eq_dec 1 target).
-            subst target. rewrite e. rewrite NatMap.gss. congruence.
-            rewrite NatMap.gso. eauto. eauto.
-         -- destruct CUR_INJP_TID as [X Y]. unfold wp'.
-            split; eauto. 
-            simpl. simpl. unfold wpj'. 
-            inv H3. simpl. unfold gw_nexttid. simpl. rewrite <- H. reflexivity.
-         -- intros. destruct (Nat.eq_dec n target).
-            subst. rewrite NatMap.gss in H0. inv H0.
-            split. reflexivity. lia.
-            rewrite NatMap.gso in H0.
-            exploit FIND_TID; eauto. eauto.
-         -- intros.
-            instantiate (1:= NatMap.set target None worldsA).
-            destruct (Nat.eq_dec n target).
-            ++ subst.
-               exists wB, None, wp'. eexists. eexists. exists li'.
-               repeat apply conj; eauto.
-               rewrite NatMap.gss. reflexivity.
-               rewrite NatMap.gss. reflexivity.
-               rewrite NatMap.gss. reflexivity.
-               econstructor; eauto.
-               rewrite NatMap.gss. reflexivity.
-               intros. congruence.
-            ++ destruct (THREADS n H0) as (wn & owan & wnp & lscn & lsan & lin & A & B & C & D & E & F & G & I & J).
-               exists wn, owan, wnp, lscn,lsan,lin. repeat apply conj; try rewrite NatMap.gso; eauto.
-               rewrite <- OTHERi; eauto. lia.
-               intros n1. specialize (J n1). subst wp'.
-               eapply gw_accg_yield_accg; eauto. simpl.
-               rewrite <- H.
-               econstructor; eauto. inv H3. econstructor; eauto.
-               inv H8. econstructor; eauto.
-               exploit FIND_TID. apply I. intros [X Y].
-               unfold gw_tid. simpl. 
-               setoid_rewrite X. lia.
-       + (*join*)
-         assert (lsc = CMulti.Returnj OpenC ls1 tar' vptr).
-         eapply foo; eauto. subst lsc. inv MS.
-         assert (get wA = wPcur). clear -GETWp CUR_GWORLD.
-         rewrite CUR_GWORLD in GETWp. inv GETWp. reflexivity. subst wPcur.
-         apply FIND_TID in GETWp as X. destruct X as [HwaTid RNGtarget].
-         destruct wA as (se0 & [se0' m0'] & se1 & [se1' sig'] & se2 & wAca & wAe).
-         simpl in GETwpc, ACCY, ACC, GETWp, HwaTid, RSLD. inv ACCY.
-         assert (ACCEJ: injp_acce (get_injp wAca) (injpw f m' tm' Hmj')).
-         { eapply injp_acc_yield_acce. rewrite <- H. inv H3.
-           econstructor; eauto. eauto. }
-         assert (ACCEE: ext_acce (extw m2 m3 Hme0) (extw tm' ttm' Hme')).
-         {
-           assert (BASE:injp_tid (get_injp wAca) = injp_tid (injpw f m' tm' Hmj')).
-           eauto. eapply ext_acc_yield_acce; eauto. inv H8. econstructor; eauto.
-           simpl. rewrite <- H in BASE. simpl in BASE.
-           erewrite <- inject_tid. 2: eauto. rewrite BASE.
-           erewrite inject_tid;eauto.
-         }
-         specialize (THREADS tar' RNG_WAIT) as THR_TAR'.
-         destruct THR_TAR' as (wBt & owAt & wPt & lsct & lsat & lit & GETWt & GETit & MSEwt & GETCt & GETAt & GETWat & MSt & GETWpt & ACCt).         
-         assert (lsct = CMulti.Final OpenC res ).   eapply foo; eauto. subst lsct.
-         inv MSt.
-         exploit ACCt. congruence. intro ACCt'.
-         rename gmem'' into m''.
-         set (qc := cr (Vint Int.one) m'). rename rs into trs.
-         set (rs := cajw_rs wAca).
-         set (rs' := Pregmap.set RAX (Vint Int.one)(Pregmap.set PC (rs RA) rs)).
-         set (trs' := Pregmap.set RAX (Vint Int.one)(Pregmap.set PC (trs RA) trs)).
-         unfold injp_w_compcert in VPTR. simpl in VPTR.
-         setoid_rewrite <- H in VPTR. simpl in VPTR.
-         exploit Mem.storev_mapped_inject.
-         2: eauto. eauto.
-         eauto. simpl in ACCt'. unfold get_injp in ACCt'.
-         unfold get_injp in H. rewrite <- H in ACCt'.
-         eapply val_inject_incr. 2: eauto. inv ACCt'.
-         inv H7. simpl. eauto.
-         intros [tm''[MEM_RES' Hmj'']].
-         set (r_a := (rs', tm'')).
-         exploit Mem.storev_extends; eauto.
-         intros [ttm'' [MEM_RES'' Hme'']].
-         set (tr_a := (trs', ttm'')).
-         set (wpj' := injpw f m'' tm'' Hmj'').
-         set (wp' := (tt,(tt, (wpj', extw tm'' ttm'' Hme'')))).
-         assert (ACCEJ2: injp_acce (get_injp wAca) wpj').
-         {
-           simpl in VPTR. destruct wAca. simpl in *.
-           destruct cajw_injp. unfold wp'. simpl in *.
-           eapply injp_acce_storev; eauto.  
-         }
-         assert (ACCEE2: ext_acce (extw m2 m3 Hme0) (extw tm'' ttm'' Hme'')).
-         { etransitivity. eauto.
-         exploit ext_acci_storev. apply MEM_RES'. apply MEM_RES''. eauto. eauto. }
-         exploit M_REPLIES; eauto.
-         instantiate (1:= (tt,(tt,(injpw f m'' tm'' Hmj'', extw tm'' ttm'' Hme'')))).
-         repeat eapply conj; simpl; eauto. 
-         instantiate (1:= tr_a). unfold tr_a. simpl.
-         { (* match_reply *)
-           eexists. split. econstructor. constructor.
-           inv WT_WA. simpl in ACCEJ2. unfold wpj' in ACCEJ2. inv ACCEJ2.
-           destruct H15 as [_ [X _]]. constructor; eauto.
-           eexists. split. econstructor. inv WT_WA. unfold sig_w_compcert in WA_SIG.
-           simpl in WA_SIG. rewrite WA_SIG. simpl. auto.
-           exists r_a. split. unfold r_a. simpl.
-           destruct wAca. simpl in *.
-           econstructor; eauto.  inv WT_WA. unfold sig_w_compcert in WA_SIG.
-           simpl in WA_SIG. rewrite WA_SIG.
-           unfold Conventions1.loc_result.
-           replace Archi.ptr64 with true. simpl. unfold rs'. rewrite Pregmap.gss. constructor. eauto.
-           intros. unfold rs'.
-           destruct r; simpl in H0; inv H0; repeat rewrite Pregmap.gso;
-             simpl; try congruence; try reflexivity.
-           constructor. simpl. intros. unfold rs', trs'.
-           setoid_rewrite Pregmap.gsspec. destr; eapply val_inject_id; eauto.
-           setoid_rewrite Pregmap.gsspec. destr; eapply val_inject_id; eauto.
-           eapply val_inject_id; eauto.
-           eapply val_inject_id; eauto. constructor.
-         }
-         intros (li' & sa' & AFT_E' & MLS').
-         specialize (get_nth_set (target-1) i li li' GETi) as SETi.
-         destruct SETi as (i' & SETi & Newi & OTHERi).
-         eexists. exists i'. split.
-         (*switch_in*)
-         eapply switch_in_join; eauto.
-         (*match*)
-         econstructor. instantiate (1:= NatMap.set target (Some wp') worldsP).
-         econstructor. simpl. 8:{  rewrite NatMap.gss. reflexivity. }
-         all: eauto.
-         -- erewrite set_nth_error_length; eauto.
-         -- intros. fold target. destruct (Nat.eq_dec 1 target).
-            subst target. rewrite e. rewrite NatMap.gss. congruence.
-            rewrite NatMap.gso. eauto. eauto.
-         -- destruct CUR_INJP_TID as [X Y].
-            split.
-            transitivity (Mem.tid (Mem.support m')). reflexivity. erewrite Mem.support_storev; eauto.
-            reflexivity.
-            inv H3. simpl.
-            rewrite <- H. simpl. unfold gw_nexttid. simpl. 
-            transitivity (Mem.next_tid (Mem.support ((Mem.yield m1 n p)))). reflexivity. erewrite Mem.support_storev; eauto.
-         -- intros. destruct (Nat.eq_dec n target).
-            subst. rewrite NatMap.gss in H0. inv H0. split.
-            unfold wp'. unfold gw_tid. simpl. erewrite <- Mem.support_storev; eauto. reflexivity. simpl. lia.
-            rewrite NatMap.gso in H0. eauto. eauto.
-         -- intros.
-            instantiate (1:= NatMap.set target None worldsA).
-            destruct (Nat.eq_dec n target).
-            ++ subst.
-               exists wB, None, wp'. eexists. eexists. exists li'.
-               repeat apply conj; try rewrite NatMap.gss; eauto.
-               econstructor; eauto. simpl. intros. congruence.
-            ++ destruct (THREADS n H0) as (wn & owan & wnp & lscn & lsan & lin & A & B & C & D & E & F & G & I & J).
-               exists wn, owan, wnp, lscn,lsan,lin. repeat apply conj; try rewrite NatMap.gso; eauto.
-               rewrite <- OTHERi; eauto. lia.
-               intros n1. specialize (J n1). simpl in n1. subst wp'. simpl in *.
-               eapply gw_accg_acci_accg. eauto.
-               rewrite <- H in HwaTid.
-               repeat apply conj; simpl; eauto. rewrite <- H.
-               eapply injp_acci_storev; eauto. instantiate (1:= Hmj'1).
-               eapply injp_acc_yield_acci; eauto.
-               inv H3. econstructor; simpl; eauto.
-               etransitivity. eapply ext_acc_yield_acci; simpl; eauto.
-               simpl. 
-               erewrite <- inject_tid. 2: eauto.
-               inversion Hmj'. inv mi_thread. inv Hms. rewrite <- H5. eauto.
-               eapply ext_acci_storev; eauto.
-               constructor.
-       + (*initial, impossible*)
-         simpl in *. exfalso. eapply NOTINIT. eauto.
-     -  (*switch to others*)
-       simpl in RANGE.
-       specialize (THREADS target RANGE) as THR_TAR.
-       destruct THR_TAR as (wB & owA & wP & lsc & lsa & li & GETW & GETi & MSEw & GETC & GETA & GETWa & MS & GETWp & ACC).
-       exploit ACC. eauto. intro ACCG.
-       inv SWITCH.
-       + (*yield*)
-         assert (lsc = CMulti.Returny OpenC ls1).
-         eapply foo; eauto. subst lsc. inv MS. simpl in *.
-         assert (wpc = wPcur). congruence. subst wpc.
-         apply FIND_TID in GETWp as X. destruct X as [HwaTid RNGtarget].
-         destruct wA as (se0 & [se0' m0'] & se1 & [se1' sig'] & se2 & wAca & wAe).
-         simpl in GETwpc, ACCY, ACC, GETWp, HwaTid, RSLD. inv ACCY.
-         inv ACCG. rewrite <- H in *. rename m5 into m2'0. rename m6 into m3'0.
-         rename m4 into m1'0.
-         assert (ACCEJ: injp_acce (injpw j m1'0 m2'0 Hmj1) (injpw f m' tm' Hmj')).
-         { eapply injp_accg_yield_acce; eauto. 
-           inv H3. econstructor; eauto. }
-         assert (ACCEE: ext_acce (extw m2'0 m3'0 Hme1) (extw tm' ttm' Hme')).
-         {
-           assert (BASE:injp_tid (injpw j m1'0 m2'0 Hmj1) = injp_tid (injpw f m' tm' Hmj')). eauto.
-           eapply ext_accg_yield_acce; eauto. inv H7. econstructor; eauto.
-           simpl. simpl in BASE.
-           erewrite <- inject_tid. 2: eauto. rewrite <- BASE.
-           erewrite inject_tid; eauto.
-         }
-         set (qc := cr Vundef m'). rename rs into trs.
-         set (rs := cajw_rs wAca).
-         set (rs' := Pregmap.set PC (rs RA) rs).
-         set (trs' := Pregmap.set PC (trs RA) trs).
-         set (r_a := (rs', tm')).
-         set (tr_a := (trs', ttm')).
-         exploit M_REPLIES; eauto.
-         instantiate (1:= (tt,(tt,(injpw f m' tm' Hmj',extw tm' ttm' Hme')))).
-         repeat apply conj; simpl; eauto.
-         instantiate (1:= tr_a). unfold tr_a.
-         { (*match_reply*)
-           eexists. split. econstructor; eauto. constructor.
-           inv WT_WA. simpl in H. inv H. inv ACCEJ.
-           destruct H16 as [_ [A _]].
-           constructor; eauto.
-           eexists. split. econstructor; eauto. inv WT_WA.
-           unfold sig_w_compcert in WA_SIG. simpl in WA_SIG.
-           rewrite WA_SIG. simpl. auto.
-           exists (r_a). unfold r_a. split. destruct wAca.
-           econstructor; eauto.
-           intros. unfold rs'.
-           destruct r; simpl in H; inv H; repeat rewrite Pregmap.gso;
-             simpl; try congruence; try reflexivity.
-           econstructor; eauto. simpl.
-           intros. unfold rs', trs'. setoid_rewrite Pregmap.gsspec.
-           destr; eapply val_inject_id; eauto.
-           constructor.
-         }
-         intros (li' & sa' & AFT_E' & MLS').
-         specialize (get_nth_set (target-1) i li li' GETi) as SETi.
-         destruct SETi as (i' & SETi & Newi & OTHERi).
-         eexists. exists i'. split.
-         (*switch_in*)
-         econstructor; eauto.
-         (*match*)
-         set (wpj' := injpw f m' tm' Hmj').
-         set (wp' := (tt,(tt,(wpj', extw tm' ttm' Hme')))).
-         econstructor. instantiate (1:= NatMap.set target (Some wp') worldsP).
-         econstructor; simpl. 8:{  rewrite NatMap.gss. reflexivity. }
-         all: eauto.
-         -- erewrite set_nth_error_length; eauto.
-         -- intros. fold target. destruct (Nat.eq_dec 1 target).
-            subst target. rewrite e. rewrite NatMap.gss. congruence.
-            rewrite NatMap.gso. eauto. eauto.
-         -- destruct CUR_INJP_TID as [X Y]. subst wp'.
-            split. reflexivity. inv H3. reflexivity.
-         -- intros. destruct (Nat.eq_dec n0 target).
-            subst. rewrite NatMap.gss in H0. inv H0.
-            split. reflexivity. lia.
-            rewrite NatMap.gso in H0. eauto. eauto.
-         -- intros.
-            instantiate (1:= NatMap.set target None worldsA).
-            destruct (Nat.eq_dec n0 target).
-            ++ subst.
-               exists wB, None, wp'. eexists. eexists. exists li'.
-               repeat apply conj; eauto.
-               rewrite NatMap.gss. reflexivity.
-               rewrite NatMap.gss. reflexivity.
-               rewrite NatMap.gss. reflexivity.
-               econstructor; eauto. rewrite NatMap.gss. reflexivity.
-               intros. congruence.
-            ++ destruct (THREADS n0 H0) as (wn & owan & wnp & lscn & lsan & lin & A & B & C & D & E & F & G & I & J).
-               exists wn, owan, wnp, lscn,lsan,lin. repeat apply conj; try rewrite NatMap.gso; eauto.
-               rewrite <- OTHERi; eauto. lia.
-               intros n2. destruct (Nat.eq_dec n0 cur).
-               subst.
-               replace wnp with  (tt, (tt, (injpw f m1 m2 Hmj, extw m2 m3 Hme0)))
-                 by congruence.
-               eapply gw_yield_acci_accg. 2: reflexivity. unfold wp', wpj'.
-               econstructor; eauto. inv H3. econstructor; eauto.
-               inv H7. econstructor; eauto.
-               apply FIND_TID in GETwpc. destruct GETwpc as [X Y]. rewrite X.
-               unfold wp', wpj', gw_tid. simpl. lia. constructor.
-               specialize (J n3).
-               eapply gw_accg_yield_accg. eauto.
-               econstructor; eauto. inv H3. econstructor; eauto.
-               inv H7. econstructor; eauto.
-               apply FIND_TID in I. destruct I as [X Y]. rewrite X.
-               unfold wp', wpj'. simpl. unfold gw_tid. simpl. lia.
-       + (*join*)
-         assert (lsc = CMulti.Returnj OpenC ls1 tar' vptr).
-         eapply foo; eauto. subst lsc. inv MS.
-         assert (wpc = wPcur). congruence. subst wpc.
-         apply FIND_TID in GETWp as X. destruct X as [HwaTid RNGtarget].
-         destruct wA as (se0 & [se0' m0'] & se1 & [se1' sig'] & se2 & wAca & wAe).
-         simpl in GETwpc, ACCY, ACC, GETWp, HwaTid, RSLD, ACCG, VPTR.
-         unfold injp_w_compcert in VPTR. simpl in VPTR.
-         exploit gw_accg_yield_acce; eauto. constructor.
-         intro ACCE. destruct ACCE as [_ [_ [ACCEJ ACCEE]]].
-         simpl in ACCEJ, ACCEE. rename rs into trs.
-         destruct wAca as [wAj sig rs]. simpl in VPTR.
-         unfold sig_w_compcert in WA_SIG. simpl in WA_SIG, ACCEJ.
-         (* get the waited thread state *)
-         specialize (THREADS tar' RNG_WAIT) as THR_TAR'.
-         destruct THR_TAR' as (wBt & owAt & wPt & lsct & lsat & lit & GETWt & GETit & MSEwt & GETCt & GETAt & GETWat & MSt & GETWpt & ACCt).         
-         assert (lsct = CMulti.Final OpenC res ).   eapply foo; eauto. subst lsct.         
-         inv MSt.
-         assert (ACCT: gw_accg wPt wPcur \/ wPcur = wPt).
-         {
-           destruct (Nat.eq_dec tar' cur). subst. right. congruence.
-           left. eapply ACCt; eauto.
-         }
-         rename gmem'' into m''.
-         set (qc := cr (Vint Int.one) m').
-         set (rs' := Pregmap.set RAX (Vint Int.one)(Pregmap.set PC (rs RA) rs)).
-         set (trs' := Pregmap.set RAX (Vint Int.one)(Pregmap.set PC (trs RA) trs)).
-         exploit Mem.storev_mapped_inject; eauto.
-         inv ACCEJ. 
-         eapply val_inject_incr. 2: eauto. simpl. eauto.
-         eapply val_inject_incr. 2: eauto.
-         {
-           destruct ACCT. inv ACCY. inv H. simpl. inv H6. eauto.
-           inv ACCY. eauto.
-         }
-         intros [tm''[MEM_RES' Hmj'']].
-         set (r_a := (rs', tm'')).
-         exploit Mem.storev_extends; eauto.
-         intros [ttm'' [MEM_RES'' Hme'']].
-         set (tr_a := (trs', ttm'')).
-         set (wpj' := injpw f m'' tm'' Hmj'').
-         set (wp' := (tt,(tt,(wpj', extw tm'' ttm'' Hme'')))).
-         
-         assert (ACCEJ': injp_acce (wAj) wpj').
-         eapply injp_acce_storev; eauto. simpl in *. inv ACCEJ. eauto.
-         assert (ACCEE' : ext_acce wAe (extw tm'' ttm'' Hme'')).
-         etransitivity. eauto. exploit ext_acci_storev. apply MEM_RES'. eauto. eauto.
-         eauto.
-         simpl in H1. inv WT_WA. simpl in ACC1. unfold rs_w_compcert in RSLD. simpl in RSLD.
-         simpl in HwaTid.
-                  
-         exploit M_REPLIES; eauto. simpl. instantiate (1:= wp').
-         repeat apply conj; eauto.
-         { instantiate (1:= tr_a). unfold tr_a.
-           eexists. split. econstructor; eauto. constructor.
-           eapply ro_acc_trans. instantiate (1:= m'). inv ACCEJ. destruct H11 as [_ [A _]].
-           constructor; eauto. unfold Mem.storev in MEM_RES. destr_in MEM_RES.
-           eapply ro_acc_store; eauto.
-           eexists. split. econstructor; eauto. constructor.
-           exists r_a. unfold r_a. split.
-           econstructor; eauto. unfold Conventions1.loc_result.
-           replace Archi.ptr64 with true. simpl. unfold rs'. rewrite Pregmap.gss. constructor. eauto.
-           intros. unfold rs'.
-           destruct r; simpl in H; inv H; repeat rewrite Pregmap.gso;
-             simpl; try congruence; try reflexivity.
-           econstructor; eauto. simpl. intros. unfold rs', trs'.
-           setoid_rewrite Pregmap.gsspec. destr; eauto. eapply val_inject_id; eauto.
-           setoid_rewrite Pregmap.gsspec. destr; eauto. constructor. }
-         intros (li' & sa' & AFT_E' & MLS').
-         specialize (get_nth_set (target-1) i li li' GETi) as SETi.
-         destruct SETi as (i' & SETi & Newi & OTHERi).
-         eexists. exists i'. split.
-         (*switch_in*)
-         eapply switch_in_join; eauto.
-         (*match*)
-         econstructor. instantiate (1:= NatMap.set target (Some wp') worldsP).
-         econstructor. simpl. 8:{  rewrite NatMap.gss. reflexivity. }
-         all: simpl; eauto.
-         -- erewrite set_nth_error_length; eauto.
-         -- intros. fold target. destruct (Nat.eq_dec 1 target).
-            subst target. rewrite e. rewrite NatMap.gss. congruence.
-            rewrite NatMap.gso. eauto. eauto.
-         -- destruct CUR_INJP_TID as [X Y].
-            split.
-            transitivity (Mem.tid (Mem.support m')). reflexivity. erewrite Mem.support_storev; eauto.
-            unfold wp', wpj'. unfold gw_tid. simpl. reflexivity.
-            inv ACCY. inv H4. unfold gw_nexttid. simpl.
-            transitivity (Mem.next_tid (Mem.support ((Mem.yield m1 n0 p)))). reflexivity.
-            erewrite Mem.support_storev; eauto.
-         -- intros. destruct (Nat.eq_dec n0 target).
-            subst. rewrite NatMap.gss in H. inv H. unfold gw_tid. simpl.
-            erewrite <- Mem.support_storev; eauto. split. reflexivity. lia.
-            rewrite NatMap.gso in H. eauto. eauto.
-         -- intros.
-            instantiate (1:= NatMap.set target None worldsA).
-            destruct (Nat.eq_dec n0 target).
-            ++ subst.
-               exists wB, None, wp'. eexists. eexists. exists li'.
-               repeat apply conj; try rewrite NatMap.gss; eauto.
-               econstructor; eauto. simpl. intros. congruence.
-            ++ destruct (THREADS n0 H) as (wn & owan & wnp & lscn & lsan & lin & A & B & C & D & E & F & G & I & J).
-               exists wn, owan, wnp, lscn,lsan,lin. repeat apply conj; try rewrite NatMap.gso; eauto.
-               rewrite <- OTHERi; eauto. lia.
-               intros n2.
-               assert (ACIJS: injp_acci (injpw f m' tm' Hmj') (injpw f m'' tm'' Hmj'')).
-               apply injp_acc_tl_i.
-               eapply injp_acc_tl_storev; eauto. inv ACCEJ. eauto.
-               exploit ext_acci_storev. apply MEM_RES'. apply MEM_RES''.
-               eauto. intro ACIES.
-               destruct (Nat.eq_dec n0 cur).
-               subst. replace wnp with wPcur by congruence.
-               eapply gw_accg_acci_accg.
-               eapply gw_acc_yield_accg. eauto.
-               simpl in ACCG.
-               apply gw_accg_neq in ACCG as NEQ.
-               inv ACCEJ. destruct H12 as [[AA BB] _]. simpl.
-               unfold gw_tid. simpl. rewrite <- BB.
-               unfold gw_tid in NEQ. simpl in NEQ. eauto.
-               repeat apply conj; simpl; eauto. constructor.
-               specialize (J n3).
-               eapply gw_accg_acci_accg.
-               eapply gw_accg_yield_accg. eauto. eauto. simpl.
-               apply FIND_TID in I. destruct I as [X Y]. rewrite X.
-               unfold gw_tid. simpl. eauto.
-               repeat apply conj; simpl; eauto. constructor.
-       + (* initial *)
-         assert (lsc = CMulti.Initial OpenC cqv).
-         eapply foo; eauto. subst lsc. inv MS.
-         assert (wpc = wPcur). congruence. subst wpc.
-         exploit ACC. eauto. intro ACCG_wB_wPcur.
-         set (wpj' := injpw f m' tm' Hmj').
-         apply FIND_TID in GETWp as X. destruct X as [HwaTid RNGtarget].
-         set (wp' := (tt,(tt,(wpj', extw tm' ttm' Hme')))).
-         exploit gw_accg_yield_acce. eauto. eauto.
-         eauto. constructor. intro ACCG1.
-         remember wB as wBi.
-         destruct wBi as (se0 & [se0' m0'] & se1 & [se1' sig'] & se2 & [wBj sig'' rsB] & wBe).
-         simpl in ACCG, ACC, GETWp, HwaTid, ACCG_wB_wPcur, ACCG1.
-         set (wB' := (se0,
-           ({| ro_symtbl := se0'; ro_mem := m' |},
-           (se1,
-             (se1', sig', (se2, ({| cajw_injp := wpj'; cajw_sg := sig''; cajw_rs := rsB |}, extw tm' ttm' Hme'))))))).
-         rename rs into trs.
+    
 
-         (*break the M_QUERIRES and MSEw*)
-         destruct M_QUERIES as [qc' [Hq1 [qc'' [Hq2 [qa'' [Hq3 Hq4]]]]]].
-         destruct cqv. inv Hq1. inv H. inv Hq2. inv H.
-         simpl in *. inv Hq3. inv Hq4. destruct H0. inv H4. rename tm into ttm. rename tm1 into tm. rename rsB into rs. simpl in H.
-         destruct ACCG1 as [_ [_ [ACCGJ ACCGE]]].
-         simpl in ACCGJ, ACCGE.
-         assert (MQ_CUR: GS.match_query cc_compcert wB'
-                           (cq cqv_vf start_routine_sig cqv_args m') (trs, ttm')).
-         {
-           subst targs tsp0. 
-           assert (Hincr :inject_incr j f).
-           inv ACCGJ. eauto. 
-           eexists. split. econstructor; eauto. constructor.
-           eapply ro_acc_sound; eauto. inv ACCGJ.
-           destruct H24 as [_ [? _]]. constructor; eauto.
-           eexists. split. econstructor; simpl; eauto.
-           exists (rs, tm'). split. simpl.
-           econstructor; simpl; eauto.
-           rewrite start_routine_loc in H9. simpl in H9. 
-           rewrite start_routine_loc. simpl.
-           eapply val_inject_list_incr; eauto.
-           intros. unfold Conventions.size_arguments in H4.
-           setoid_rewrite start_routine_loc in H4. simpl in H4. inv H4. extlia.
-           inv ACCGJ. inv H15.
-           econstructor. simpl. apply H25. eauto.
-           inv ACCGJ. inv H16. econstructor. destruct H25 as [[_ B] _]. congruence.
-           econstructor.  red. unfold Conventions.size_arguments.
-           rewrite start_routine_loc. simpl. auto.
-           constructor. simpl. eauto.
-           split; eauto. constructor.
-         }
-         destruct MSEw as (A & B & C & D). inv A. inv B. inv C.
-         assert (MSEw' : GS.match_senv cc_compcert wB' se tse).
-         {
-           split. constructor. reflexivity.
-           split; constructor. reflexivity.
-           inv ACCGJ. constructor. eapply Genv.match_stbls_incr_noglobal; eauto.
-           destruct H27 as [P [Q R]]. eauto.
-           destruct H28 as [P [Q R]]. eauto.
-           reflexivity.
-         }
-         specialize (fsim_lts se tse wB' MSEw' valid_se) as FSIM.
-         inversion FSIM.
-         clear fsim_simulation fsim_match_final_states fsim_match_external.
-         exploit fsim_match_initial_states.  eauto. eauto. eauto.
-         intros (li' & ls' & INIT & MLS').
-          specialize (get_nth_set (target-1) i li li' GETi) as SETi.
-         destruct SETi as (i' & SETi & Newi & OTHERi).
-         eexists. exists i'. split.
-         (* switin_in_initial *)
-         eapply switch_in_initial. eauto. eauto. eauto.
-     (* match_states *)
-         econstructor. instantiate (1:= NatMap.set target (Some wp') worldsP).
-         econstructor. 6:{ instantiate (2:= NatMap.set target (Some wB') worldsB).
-         rewrite NatMap.gso. eauto. congruence. }
-         all: simpl; eauto. erewrite set_nth_error_length; eauto.
-         intros. destruct (Nat.eq_dec 1 target). subst. congruence.
-         rewrite NatMap.gso. eauto. eauto.
-         intros. destruct (Nat.eq_dec n0 target) in H0. subst.
-         rewrite NatMap.gss in H5. inv H5.
-         split; reflexivity. 
-         rewrite NatMap.gso in H5. eauto. eauto.
-         rewrite NatMap.gss. reflexivity.
-         unfold wp'. simpl. split. eauto.
-         destruct CUR_INJP_TID as [X Y]. inv ACCY.
-         unfold gw_nexttid. simpl. inv H8. eauto.
-         intros. destruct (Nat.eq_dec n0 target). subst.
-         rewrite NatMap.gss in H4.
-         inv H4. split. reflexivity. lia.
-         rewrite NatMap.gso in H4. eauto. eauto.
-         intros. instantiate (1:= worldsA).
-         destruct (Nat.eq_dec n0 target). subst.
-         exists wB', None, wp'. eexists. eexists. exists li'.
+       
 
-         destruct MSEw' as (AA & BB & CC & DD).
-         repeat apply conj; try rewrite NatMap.gss; eauto.
-         econstructor. red. eauto.
-         intros. congruence.
-         destruct (THREADS n0 H4) as (wn & owan & wnp & lscn & lsan & lin & A & B & C & D & E & F & G & I & J).
-         exists wn, owan, wnp, lscn,lsan,lin. repeat apply conj; try rewrite NatMap.gso; eauto.
-         rewrite <- OTHERi; eauto. lia.
-         intros n2.
-         apply gw_accg_neq in ACCG as GTID. unfold gw_tid in GTID. simpl in GTID.
-         assert (TTID: Mem.tid (Mem.support m) = Mem.tid (Mem.support m')).
-         inv ACCGJ. destruct H28 as [[AA BB] _]. eauto.
-         destruct (Nat.eq_dec n0 cur).
-         subst. replace wnp with wPcur by congruence.
-         eapply gw_acc_yield_accg. eauto. simpl. 
-         unfold gw_tid. simpl. rewrite <- TTID. lia.
-         specialize (J n3).
-         eapply gw_accg_yield_accg. eauto. eauto.
-         apply FIND_TID in I. destruct I as [X Y]. rewrite X.
-         unfold gw_tid. simpl. rewrite <- TTID. lia.
-   Qed.
-    *)
-
-
+   Lemma local_plus_c : forall gs t sc1 sc2,
+        Plus (OpenC se) sc1 t sc2 ->
+        fst (CMulti.threads OpenC gs) = None ->
+        NatMap.get (CMulti.cur_tid OpenC gs) (CMulti.threads OpenC gs)  = Some (CMulti.Local OpenC sc1) ->
+        plus (CMulti.step OpenC) (CMulti.globalenv OpenC) gs t (CMulti.update_cur_thread OpenC gs (CMulti.Local OpenC sc2)).
+    Proof.
+      intros. inv H.
+      econstructor; eauto.
+      econstructor. eauto. eauto. eauto.
+      set (gs' := CMulti.update_thread OpenC gs (CMulti.cur_tid OpenC gs) (CMulti.Local OpenC s2)).
+      assert (EQ: CMulti.update_cur_thread OpenC gs (CMulti.Local OpenC sc2) = CMulti.update_cur_thread OpenC gs' (CMulti.Local OpenC sc2)).
+      unfold gs'. unfoldC. rewrite NatMap.set2.
+      reflexivity.
+      rewrite EQ.
+      eapply local_star_c; eauto.
+      unfold gs'. simpl. rewrite NatMap.gss. reflexivity.
+    Qed.
 (*
     Lemma local_plus : forall gs t sa1 sa2,
-        Plus (OpenA tse) sa1 t sa2 ->
+        lus (OpenA tse) sa1 t sa2 ->
         fst (threads OpenA gs) = None ->
         NatMap.get (cur_tid OpenA gs) (threads OpenA gs)  = Some (Local OpenA sa1) ->
         plus (step OpenA) (globalenv OpenA) gs t (update_cur_thread OpenA gs (Local OpenA sa2)).
-    Proof.
+    Proo
       intros. inv H.
       econstructor; eauto.
       econstructor. eauto. eauto. eauto.
@@ -1983,76 +796,272 @@ Admitted
       eapply local_star; eauto.
       unfold gs'. simpl. rewrite NatMap.gss. reflexivity.
     Qed.
-*)
+ *)
+    Lemma trans_pthread_create__start_routine: forall q_ptc r_ptc q_str qc_ptc rc_ptc qc_str wA,
+        query_is_pthread_create_asm OpenA q_ptc r_ptc q_str ->
+        query_is_pthread_create OpenC qc_ptc rc_ptc qc_str ->
+        GS.match_query cc_compcert wA qc_ptc q_ptc ->
+        GS.match_senv cc_compcert wA se tse ->
+        exists gw wA',
+            gw_accg (get wA') gw /\
+            (forall w, gw_accg w (get wA) -> gw_accg w gw) /\
+            (get wA) o-> gw /\
+            gw_nexttid gw = S (gw_nexttid (get wA)) /\
+                           GS.match_reply cc_compcert (set wA gw) rc_ptc r_ptc /\
+                           GS.match_query cc_compcert wA' qc_str q_str /\
+                           GS.match_senv cc_compcert wA' se tse /\
+                           worlds_ptc_str (cainjp_w_compcert wA) (cainjp_w_compcert wA').
+    Proof.
+      intros until wA. intros Hca Hcc MQ MSE.
+      inv Hca. inv Hcc.
+      destruct wA as (se0 & [se0' m0'] & se1 & [se1' sig'] & se2 & w_cap & w_e).
+      destruct MQ as [q1' [Hqr [q1'' [Hqw [qa' [Hqca Hqe]]]]]].
+      inv Hqr. inv Hqw. simpl in H. destruct H0. simpl in H0. inv H0. simpl in H1.
+      inv Hqca. inv Hqe. destruct H2 as [PCN Hme].
+      inv Hme. clear Hm4. rename Hm3 into Hme.
+      subst tvf targs. rewrite pthread_create_locs in H5. simpl in H5.
+      inv H5. inv H17. inv H18. inv H19.
+      destruct MSE as [EQ1 [EQ2 [MSE EQ3]]].
+      inv EQ1. inv EQ2. inv EQ3. inv H2. inv H3. simpl in H0.
+      rename m into ttm. rename m1 into ttm1.
+      rename m0 into m. rename m2 into m1. rename m3 into ttm3.
+      case (Mem.thread_create tm) as [tm1 id] eqn:MEM_CREATE'.
+      exploit thread_create_inject; eauto. intros [Hm1' eqid]. subst id.
+      assert (exists b_t' ofs_t', rs RDI = Vptr b_t' ofs_t').
+      inv H11. eauto. destruct H2 as [b_t' [ofs_t' RDIVAL]].
+      assert (exists b_arg' ofs_arg', rs RDX = Vptr b_arg' ofs_arg').
+      inv H13. eauto. destruct H2 as [b_arg' [ofs_arg' RDXVAL]].
+      assert (TP1: Mem.range_prop tid (Mem.support tm1)).
+      {
+        inv P0. constructor. auto. erewrite <- inject_next_tid; eauto.
+      }
+      set (tm2 := Mem.yield tm1 tid TP1).
+      case (Mem.alloc tm2 0 0 ) as [tm3 sp0] eqn:DUMMY.
+      assert (TP2: Mem.range_prop (Mem.tid (Mem.support tm)) (Mem.support tm3)).
+      {
+        generalize (Mem.tid_valid (Mem.support tm)). intro.
+        constructor; eauto. lia.
+        apply Mem.support_alloc in DUMMY. rewrite DUMMY. simpl.
+        unfold Mem.next_tid, sup_incr, Mem.sup_yield. simpl.
+        rewrite Mem.update_list_length. inv MEM_CREATE'. simpl.
+        rewrite app_length. simpl. lia.
+      }
+     set (tm4 := Mem.yield tm3 (Mem.tid (Mem.support tm)) TP2).
+     
+     set (m2 := Mem.yield m1 tid P0).
+     assert (Hm'2 : Mem.inject j m2 tm2).
+     eapply yield_inject. eauto.
+     assert (Hmq: Mem.inject j m2 tm3).
+     eapply Mem.alloc_right_inject; eauto.
+     assert (Hmr: Mem.inject j m1 tm4).
+     {
+       inv Hmq. constructor; eauto.
+       + inv mi_thread. constructor; eauto.
+         inv Hms. constructor; eauto. simpl. inv MEM_CREATE0.
+         simpl. eapply inject_tid; eauto.
+       + inv mi_inj. constructor; eauto.
+     }
+     (** similarly we need Mem.extends tm'4 ttm'4*)
+     assert (Hme1: Mem.extends tm1 ttm1).
+     {
+       clear - Hme MEM_CREATE' MEM_CREATE.
+       unfold Mem.thread_create in *. inv MEM_CREATE'.
+       inv MEM_CREATE. inv Hme.
+       constructor; simpl; eauto. congruence.
+       inv mext_inj. constructor; eauto.
+     }
+     assert (tid = new_tid).
+     {
+       clear -Hme MEM_CREATE' MEM_CREATE.
+       unfold Mem.thread_create in *. inv MEM_CREATE'.
+       inv MEM_CREATE. inv Hme. rewrite mext_sup. reflexivity.
+     }
+     subst new_tid.
+     set (ttm2 := Mem.yield ttm1 tid P1).
+     assert (Hme2: Mem.extends tm2 ttm2).
+     apply yield_extends; eauto.
+     exploit Mem.alloc_extends. apply Hme2. eauto. reflexivity. reflexivity.
+     intros (ttm3' & DUMMY2 & Hmqe). fold ttm2 in MEM_ALLOCSP.
+     setoid_rewrite MEM_ALLOCSP in DUMMY2. inv DUMMY2. rename ttm3' into ttm3.
+     set (ttm4 := Mem.yield ttm3 (Mem.tid (Mem.support ttm)) P2).
+     assert (Hmre: Mem.extends tm4 ttm4).
+     apply yield_extends; eauto. inv Hme. congruence.
+     rename rs into trs. rename rs0 into rs.
+     set (rs_q := rs # PC <- (rs RSI) # RDI <- (rs RDX) # RSP <- (Vptr sp0 Ptrofs.zero)).
+     set (rs_r := rs # PC <- (rs RA) # RAX <- (Vint Int.one)).
+     set (trs_q := trs # PC <- (trs RSI) # RDI <- (trs RDX) # RSP <- (Vptr sp0 Ptrofs.zero)).
+     set (trs_r := trs # PC <- (trs RA) # RAX <- (Vint Int.one)).
+     rename H0 into RSLD. simpl in RSLD.
+     (* eapply lessdef_trans in PCVAL as PCVAL'; eauto.
+     eapply lessdef_trans in RSIVAL as RSIVAL'; eauto.
+     eapply lessdef_trans in RDIVAL as RDIVAL'; eauto.
+     eapply lessdef_trans in RDXVAL as RDXVAL'; eauto. *)
+     inv H.
+     exists (tt, (tt, (injpw j m1 tm4 Hmr, extw tm4 ttm4 Hmre))).
+     exists (se, ((row se m2), (se, (se, start_routine_sig, (tse,((cajw (injpw j m2 tm3 Hmq) start_routine_sig rs_q) , extw tm3 ttm3 Hmqe))) ))).
+     assert (UNC23: Mem.unchanged_on (fun _ _ => True) tm2 tm3). eapply Mem.alloc_unchanged_on. eauto.
+     assert (UNC23': Mem.unchanged_on (fun _ _ => True) ttm2 ttm3). eapply Mem.alloc_unchanged_on. eauto.
+     apply Mem.support_alloc in DUMMY as HSUP. rename MEM_ALLOCSP into DUMMY2.
+     apply Mem.support_alloc in DUMMY2 as HSUP2. simpl.
+     assert (ROACCR1 : ro_acc m m1). eapply ro_acc_thread_create; eauto.
+     assert (ROACCQ1: ro_acc m m2). eapply ro_acc_trans. eauto. eapply ro_acc_yield; eauto. reflexivity.
+     assert (ROACCQ2: ro_acc tm tm3).
+     eapply ro_acc_trans. eapply ro_acc_thread_create; eauto.
+     eapply ro_acc_trans. eapply ro_acc_yield. 
+     instantiate (1:= tm2). reflexivity. eapply ro_acc_alloc; eauto.
+     assert (ROACCR2: ro_acc tm tm4). eapply ro_acc_trans. eauto. eapply ro_acc_yield; eauto. reflexivity.
+     assert (ROACCQ3: ro_acc ttm ttm3).
+      eapply ro_acc_trans. eapply ro_acc_thread_create; eauto.
+     eapply ro_acc_trans. eapply ro_acc_yield. 
+     instantiate (1:= ttm2). reflexivity. eapply ro_acc_alloc; eauto.
+     assert (ROACCR3: ro_acc ttm ttm4). eapply ro_acc_trans. eauto. eapply ro_acc_yield; eauto. reflexivity.
+     assert (SINC1: Mem.sup_include (Mem.support tm) (Mem.support tm4)).
+     { inv ROACCR2. eauto. }
+     assert (SINC2: Mem.sup_include (Mem.support ttm) (Mem.support ttm4)).
+     { inv ROACCR3. eauto. } 
+     repeat apply conj.
+     - (** accg *)
+       simpl. econstructor.
+       econstructor; eauto; try red; intros; try congruence; eauto.
+       split. split; eauto. inv MEM_CREATE0. simpl. generalize (Mem.tid_valid (Mem.support m)). intro. unfold Mem.next_tid. simpl. lia.
+       inv MEM_CREATE0. constructor; eauto. simpl. red. intros. eauto with mem.
+       intros. reflexivity.
+       split. split; eauto.
+       simpl. erewrite Mem.support_alloc; eauto. simpl. inv MEM_CREATE'. simpl.
+       generalize (Mem.tid_valid (Mem.support tm)). intro. unfold Mem.next_tid. lia.
+       constructor; eauto. simpl. red. intros. eauto with mem. intros. reflexivity.
+       {
+         unfold tm4, ttm4.
+         econstructor; simpl.
+         erewrite Mem.support_alloc; eauto. simpl. inv MEM_CREATE'.
+         generalize (Mem.tid_valid (Mem.support tm)). intro. unfold Mem.next_tid. lia.
+         erewrite Mem.support_alloc; eauto. simpl. inv MEM_CREATE.
+         generalize (Mem.tid_valid (Mem.support ttm)). intro. unfold Mem.next_tid. lia.
+         red. intros. eauto with mem. red. intros. eauto with mem.
+         red. intros. eauto with mem. red. intros. eauto with mem.
+       }
+     - intros. inv H. inv MEM_CREATE0. inv MEM_CREATE'. constructor. 
+       unfold injp_gw_compcert.
+       simpl. inv H17.
+       assert (ROACC: ro_acc m3 tm4). { eapply ro_acc_trans. 2: eauto.
+       destruct H28 as [_ [A _]]. constructor; eauto. }
+       econstructor; eauto.
+       + inv ROACC. eauto.
+       + inv ROACC. eauto.
+       + destruct H27 as [[A B] C]. constructor; simpl. split. unfold Mem.next_tid, Mem.sup_create in *. simpl. rewrite app_length. simpl. lia.
+         lia. inv C. constructor; simpl. eapply Mem.sup_include_trans. eauto. red. intros. rewrite <- Mem.sup_create_in. auto.
+         intros. etransitivity. eauto. reflexivity. intros. etransitivity. reflexivity. eauto.
+       + destruct H28 as [[A B] C]. constructor; simpl. split. etransitivity. eauto.
+         unfold Mem.next_tid, Mem.sup_yield. simpl.
+         rewrite HSUP. simpl. rewrite Mem.update_list_length. rewrite app_length. simpl. lia. lia.
+         inv C. constructor; simpl. eapply Mem.sup_include_trans. eauto. red. intros. rewrite <- Mem.sup_yield_in.
+         rewrite HSUP. apply Mem.sup_incr_in2. simpl. rewrite <- Mem.sup_yield_in, <- Mem.sup_create_in. eauto.
+         intros. etransitivity. eauto. transitivity (Mem.perm tm2 b ofs k p). reflexivity.
+         transitivity (Mem.perm tm3 b ofs k p). 2: reflexivity. inv UNC23. apply unchanged_on_perm0; eauto.
+         red. simpl. rewrite <- Mem.sup_yield_in, <- Mem.sup_create_in. eauto.
+         intros. inv UNC23. rewrite unchanged_on_contents0; eauto. apply unchanged_on_perm in H0; eauto with mem.
+       + inv H21. inv ROACCR2. inv ROACCR3.
+         constructor; simpl. eauto. eauto.
+         eapply Mem.sup_include_trans; eauto.
+         eapply Mem.sup_include_trans; eauto.
+         eapply max_perm_decrease_trans. apply MPD1. eauto. eauto.
+         eapply max_perm_decrease_trans. apply MPD2. eauto. eauto.
+     - auto.
+     - auto.
+     - simpl. inv MEM_CREATE0. inv MEM_CREATE'.
+       constructor; simpl; eauto; try red; intros; simpl in *; try congruence; eauto.
+       assert (Mem.loadbytes tm3 b ofs n = Some bytes). eauto.
+       erewrite Mem.loadbytes_unchanged_on_1 in H17. 2: eauto. eauto.
+       red. simpl. rewrite <- Mem.sup_yield_in, <- Mem.sup_create_in. eauto.
+       intros. simpl. reflexivity.
+       assert (Mem.perm tm3 b ofs Max p). eauto.
+       exploit Mem.perm_unchanged_on_2; eauto. reflexivity.
+       red. simpl. rewrite <- Mem.sup_yield_in, <- Mem.sup_create_in. eauto.
+       split. split; simpl; eauto. rewrite app_length. simpl. lia. constructor; simpl; eauto. 
+       red. intros. rewrite <- Mem.sup_create_in. auto. intros. reflexivity.
+       split. split; simpl; eauto. rewrite HSUP. simpl. rewrite Mem.update_list_length. rewrite app_length. simpl. lia.
+       constructor; eauto.
+       intros. unfold tm4. transitivity (Mem.perm tm2 b ofs k p). reflexivity.
+       transitivity (Mem.perm tm3 b ofs k p). 2: reflexivity.
+       inv UNC23. apply unchanged_on_perm; eauto. red. simpl. rewrite <- Mem.sup_yield_in, <- Mem.sup_create_in. eauto.
+       intros. transitivity (  Maps.ZMap.get ofs (NMap.get (Maps.ZMap.t memval) b (Mem.mem_contents tm2))).
+       2: reflexivity.
+       inv UNC23. apply unchanged_on_contents; eauto.
+     - simpl. constructor; eauto. inv ROACCR2. eauto. inv ROACCR3. eauto.
+     - unfold gw_nexttid. simpl. inv MEM_CREATE0. simpl. unfold Mem.sup_create. unfold Mem.next_tid.
+       simpl. rewrite app_length. simpl. lia.
+     - econstructor; eauto.
+       split. econstructor; eauto. constructor. eauto.
+       eexists. split. econstructor; eauto. 
+       unfold pthread_create_sig. simpl. auto.
+       exists (rs_r, tm4). split. econstructor; eauto.
+       unfold pthread_create_sig. simpl.
+       unfold Conventions1.loc_result. replace Archi.ptr64 with true. simpl.
+       unfold rs_r. rewrite Pregmap.gss. constructor. eauto.
+       intros. unfold rs_r. rewrite !Pregmap.gso; eauto.
+       destruct r; simpl in H1; simpl; congruence.
+       destruct r; simpl in H; simpl; congruence.
+       constructor; simpl; eauto.
+       intros. unfold rs_r. unfold trs_r.
+       setoid_rewrite Pregmap.gsspec. destr. constructor.
+       setoid_rewrite Pregmap.gsspec. destr. eauto. eauto. fold ttm4. econstructor.
+     - eexists. split. econstructor; eauto. econstructor.
+       eapply ro_acc_sound; eauto.
+       eexists. split. econstructor; eauto. simpl. intuition auto.
+       exists (rs_q, tm3). split.
+       econstructor; eauto. rewrite start_routine_loc. simpl.
+       constructor. unfold rs_q. rewrite Pregmap.gso; try congruence.
+       rewrite Pregmap.gss. eauto.
+       constructor. unfold Conventions.size_arguments.
+       rewrite start_routine_loc. simpl. intros. inv H. extlia.
+       unfold rs_q. rewrite Pregmap.gss. constructor.
+       eapply Hvalid; eauto. eapply Hlocal; eauto.
+       econstructor. unfold Conventions.tailcall_possible, Conventions.size_arguments.
+       rewrite start_routine_loc. simpl. reflexivity. congruence.
+       constructor; eauto. simpl. unfold rs_q, trs_q. intros.
+       setoid_rewrite Pregmap.gsspec. destr. apply val_inject_id. constructor.
+       setoid_rewrite Pregmap.gsspec. destr. rewrite <- RS_RDX. eauto. eauto.
+       setoid_rewrite Pregmap.gsspec. destr. rewrite <- RS_RSI. eauto. eauto.
+       split. unfold rs_q. rewrite Pregmap.gso; try congruence.
+       rewrite Pregmap.gso; try congruence. rewrite Pregmap.gss. inv H5. congruence.
+       constructor.
+     - constructor. reflexivity.
+     - constructor. reflexivity.
+     - inv MSE. constructor; eauto. inv ROACCQ1. eapply Mem.sup_include_trans; eauto.
+     - reflexivity.
+     - econstructor; eauto. reflexivity.
+   Qed.
     
-   Lemma Concur_BSimP : Closed.bsim_properties ConcurC ConcurA global_index global_order match_states.
-      constructor. auto.
-      - eapply global_index_wf.
-      - eapply concur_initial_states_exist; eauto.
-      - eapply concur_initial_states.
-      - eapply concur_final_states.
-      -
-                                                                                               
-
-        (* progress *)
-        intros. exploit H0; eauto.
-        eapply star_refl.  intros [[r F]| [t [s1'' S]]].
-        + (*final*)
-          inv F. inv H. inv H4. simpl in H1, H2. unfold CMulti.get_cur_thread in H2. simpl in H2.
-          specialize (THREADS cur CUR_VALID) as THR_CUR. 
-          destruct THR_CUR as (wB & owA & wP & lsc & lsa & li & GETW & GETi & MSEw & GETC & GETA & GETWa & MS & GETWp & ACC).
-          assert (lsc = CMulti.Local OpenC ls).
-          eapply foo; eauto. subst lsc. inv MS.
-          specialize (bsim_lts se tse wB MSEw valid_se) as BSIM.
-          inversion BSIM.
-          exploit bsim_progress. eauto.
-          { (*safe lemma, to be moved out *)
-            red. red in H0. intros. exploit H0.
-            eapply local_star_c; eauto. simpl.
-            intros [[r1 F]| [t [s1'' S]]].
-            - inv F.
-              unfold CMulti.get_cur_thread, CMulti.update_cur_thread, CMulti.get_thread,
-                CMulti.update_thread in H5.
-              simpl in H5.  rewrite NatMap.gss in H5. inv H5.
-              left. eauto.
-            - inv S; unfold CMulti.get_cur_thread, CMulti.update_cur_thread, CMulti.get_thread,
-                CMulti.update_thread in H1;
-              simpl in H1.
-              + rewrite NatMap.gss in H1. inv H1. right. right. eauto.
-              + rewrite NatMap.gss in H1. inv H1. right. left. eauto. 
-              + inv H1.
-                -- unfold CMulti.get_cur_thread, CMulti.update_cur_thread, CMulti.get_thread,
-                     CMulti.update_thread in GET_C; simpl in GET_C; rewrite NatMap.gss in GET_C. inv GET_C.
-                   right. left. eauto.
-                -- unfold CMulti.get_cur_thread, CMulti.update_cur_thread, CMulti.get_thread,
-                     CMulti.update_thread in GET_C; simpl in GET_C; rewrite NatMap.gss in GET_C. inv GET_C.
-                   right. left. eauto.
-                -- unfold CMulti.get_cur_thread, CMulti.update_cur_thread, CMulti.get_thread,
-                     CMulti.update_thread in GET_C; simpl in GET_C; rewrite NatMap.gss in GET_C. inv GET_C.
-                   left. eauto.
-          }
-          intros [[r1 F]| [[q E]|[t [sa' S]]]].
-          -- 
-          intros []
-      - (* step *)
-        intros. inv H.
+   Lemma concur_step :
+     forall (s2 : Closed.state ConcurA) (t : trace) (s2' : Closed.state ConcurA),
+       Closed.step ConcurA (Closed.globalenv ConcurA) s2 t s2' ->
+       forall (i : global_index) (s1 : Closed.state ConcurC),
+         match_states i s1 s2 ->
+         Closed.safe ConcurC s1 ->
+         exists (i' : global_index) (s1' : Closed.state ConcurC),
+           (plus (Closed.step ConcurC) (Closed.globalenv ConcurC) s1 t s1' \/
+              star (Closed.step ConcurC) (Closed.globalenv ConcurC) s1 t s1' /\ global_order i' i) /\
+             match_states i' s1' s2'.
+   Proof.
+      intros. inv H.
         + (* Local *)
-          inv H1. inv H. simpl in *.
+          inv H0. inv H. unfoldA_in H2.
           specialize (THREADS cur CUR_VALID) as THR_CUR.
           destruct THR_CUR as (wB & owA & wP & lsc & lsa & li & GETW & GETi & MSEw & GETC & GETA & GETWa & MS & GETWp & ACC).
-          assert (lsc = CMulti.Local OpenC ls1).
-          eapply foo; eauto. subst lsc. inv MS.
-          specialize (fsim_lts se tse wB MSEw valid_se) as FSIM.
-          inversion FSIM.
-          clear fsim_match_initial_states
-            fsim_match_final_states fsim_match_external.
-          exploit fsim_simulation; eauto. intros (li' & s2' & STEP & MATCH).
+          assert (lsa = AsmMulti.Local OpenA ls1).
+          eapply foo; eauto. subst lsa. inv MS.
+          specialize (bsim_lts se tse wB MSEw valid_se) as BSIM.
+          inversion BSIM.
+          clear bsim_match_initial_states
+            bsim_match_final_states bsim_match_external.
+          exploit bsim_simulation; eauto. eapply safe_concur_single; eauto.
+          intros (li' & s2' & STEP & MATCH).
           specialize (get_nth_set (cur-1) i li li' GETi) as SETi.
           destruct SETi as (i' & SETi & Newi & OTHERi). exists i'.
           assert (wP = wPcur). congruence. subst.
           destruct STEP.
           -- eexists. split. left.
-             eapply local_plus; eauto. unfold update_cur_thread.
+             eapply local_plus_c; eauto. unfold update_cur_thread.
              {
                simpl. econstructor. econstructor. simpl; eauto. simpl.
                erewrite set_nth_error_length; eauto. eauto.
@@ -2063,20 +1072,21 @@ Admitted
                eauto. eauto.
                instantiate (2:= worldsP). simpl. eauto.
                destruct CUR_INJP_TID. simpl. split; eauto.
-               eauto. eauto.
+               eauto. eauto. simpl. eauto.
                intros. instantiate (1:= worldsA).
                destruct (Nat.eq_dec n cur).
                - subst.
-                 exists wB, None, wPcur, (CMulti.Local OpenC ls2), (Local OpenA s2'), li'.
+                 exists wB, None, wPcur, (CMulti.Local OpenC s2'), (Local OpenA ls2), li'.
                  repeat apply conj; eauto. rewrite NatMap.gss. reflexivity.
                  rewrite NatMap.gss. reflexivity. simpl. constructor. eauto.
                - (* clear - THREADS H3 OTHERi n0. *)
-                 destruct (THREADS n H3) as (wn & owan & wnp & lscn & lsan & lin & A & B & C & D & E & F & G & I & J).
+                 simpl in *.
+                 destruct (THREADS n H4) as (wn & owan & wnp & lscn & lsan & lin & A & B & C & D & E & F & G & I & J).
                  exists wn, owan, wnp, lscn,lsan,lin. repeat apply conj; eauto. rewrite <- OTHERi; eauto. lia.
                  rewrite NatMap.gso. simpl. eauto. lia.
                  rewrite NatMap.gso. simpl. eauto. lia.
              }
-          -- destruct H. eexists. split. right. split. eapply local_star; eauto.
+          -- destruct H. eexists. split. right. split. eapply local_star_c; eauto.
              eapply global_order_decrease; eauto.
              {
                simpl. econstructor. econstructor. simpl; eauto. simpl.
@@ -2085,48 +1095,113 @@ Admitted
                intros. destruct (Nat.eq_dec 1 cur). subst.
                rewrite NatMap.gss. congruence.
                rewrite NatMap.gso; eauto.
-               eauto. eauto. eauto. eauto. eauto. eauto.
+               eauto. eauto. eauto. eauto. eauto. eauto. simpl. eauto.
                intros.
                destruct (Nat.eq_dec n cur).
                - subst.
-                 exists wB, None, wPcur, (CMulti.Local OpenC ls2), (Local OpenA s2'), li'.
+                 exists wB, None, wPcur, (CMulti.Local OpenC s2'), (Local OpenA ls2), li'.
                  repeat apply conj; eauto. rewrite NatMap.gss. reflexivity.
                  rewrite NatMap.gss. reflexivity. simpl. constructor. eauto.
                - (* clear - THREADS H3 OTHERi n0. *)
-                 destruct (THREADS n H4) as (wn & ownA & wp & lscn & lsan & lin & A & B & C & D & E & F & G & I & J).
+                 simpl in *.
+                 destruct (THREADS n H5) as (wn & ownA & wp & lscn & lsan & lin & A & B & C & D & E & F & G & I & J).
                  exists wn, ownA, wp, lscn,lsan,lin. repeat apply conj; eauto. rewrite <- OTHERi; eauto. lia.
                  rewrite NatMap.gso. simpl. eauto. lia.
                  rewrite NatMap.gso. simpl. eauto. simpl. lia.
              }
         + (* pthread_create *)
-          inv H0. inv H. subst.
+           inv H0. inv H. subst.
           specialize (THREADS cur CUR_VALID) as THR_CUR.
           destruct THR_CUR as (wB & owA & wP & lsc & lsa & li & GETW & GETi & MSEw & GETC & GETA &GETWa & MS & GETWp & ACC).
-          assert (lsc = CMulti.Local OpenC ls).
-          eapply foo; eauto. subst lsc. inv MS.
-          specialize (fsim_lts se tse wB MSEw valid_se) as FSIM.
-          inversion FSIM.
-          clear fsim_match_initial_states
-            fsim_match_final_states fsim_simulation.
-          exploit fsim_match_external. eauto. eauto.
-          intros (wA & qa_ptc & AT_PTC & APP & MQ_PTC & MS & MR).
+          assert (lsa = AsmMulti.Local OpenA ls).
+          eapply foo; eauto. subst lsa. inv MS.
+          specialize (bsim_lts se tse wB MSEw valid_se) as BSIM.
+          inversion BSIM.
+          clear bsim_match_initial_states
+            bsim_match_final_states bsim_simulation.
+          exploit bsim_match_external. eauto. eapply safe_concur_single; eauto. eauto.
+          intros (wA & s1' & qc_ptc & Hstar1 & AT_PTC & APP & MQ_PTC & MS & MR).
+          
+          (*exploit the safe property of ClosedC to get a after_external
+            all steps except for pthread_create should be ruled out *)
+
+          assert (exists rc_ptc qc_str s1'k,
+                     query_is_pthread_create OpenC qc_ptc rc_ptc qc_str /\
+                     after_external (OpenC se) s1' rc_ptc s1'k).
+          { specialize (determinate_big_C se) as DetC.
+            exploit H1. eapply local_star_c; eauto.
+            intros [[r Hr]|[t [s'' S]]].
+            - inv Hr. unfoldC_in H5. subst. unfoldC_in H6. rewrite NatMap.gss in H6.
+              inv H6. inv DetC. exfalso. eauto. 
+            - inv S; unfoldC_in H; try rewrite NatMap.gss in H.
+              + inv H. inv DetC. exfalso. eapply sd_big_at_external_nostep; eauto.
+              + inv H. inv DetC. exploit sd_big_at_external_determ. apply H6. apply AT_PTC.
+                intro. subst. eauto.
+                (* assert (rc_ptc = r_ptc0).
+                { clear - H9 PTR_TO_STR_ASM.
+                  inv H9. inv PTR_TO_STR_ASM.
+                  rewrite MEM_CREATE in MEM_CREATE0. inv MEM_CREATE0. reflexivity.
+                }
+                subst. eauto. *)
+              + inv H; unfoldC_in H6; unfoldC_in GET_C; rewrite NatMap.gss in GET_C; inv GET_C.
+                -- inv DetC.  exploit sd_big_at_external_determ. apply AT_PTC. apply AT_E.
+                   intro. subst. exfalso. (* clear - Q_YIE H4 AT_E MQ_PTC MS bsim_order. *)
+                   inv H4. inv Q_YIE. 
+                   (* Lemma cc_compcert_mq_PCinj : forall b sg args m rs tm w,
+                       GS.match_query cc_compcert (cq (Vptr b Ptrofs.zero sg args m)) (rs,tm) -> *)
+                   destruct wA as (se0 & [se0' m0'] & se1 & [se1' sig'] & se2 & w_cap & w_e).
+                   destruct MQ_PTC as [q1' [Hqr [q1'' [Hqw [qa' [Hqca Hqe]]]]]].
+                   inv Hqr. inv Hqw. simpl in H1. destruct H2.
+                   inv Hqca. inv Hqe. destruct H9 as [PCN Hme].
+                   inv Hme. clear Hm4. rename Hm3 into Hme.
+                   subst tvf targs.
+                   destruct MS as [EQ1 [EQ2 [MSE EQ3]]].
+                   inv EQ1. inv EQ2. inv EQ3. inv H9. inv H10. simpl in H2.
+                   inv MSE. inv H13. generalize (H2 PC). intro. rewrite <- H11 in H9. inv H9. inv H27.
+                   rewrite RS_PC in H24. inv H24.
+                   inv H18. exploit mge_symb; eauto. intro. apply H9 in FINDPTC.
+                   apply Genv.find_invert_symbol in FINDPTC.
+                   apply Genv.find_invert_symbol in H.
+                   unfold se in FINDPTC.
+                   setoid_rewrite FINDPTC in H. inv H.
+                -- inv DetC.  exploit sd_big_at_external_determ. apply AT_PTC. apply AT_E.
+                   intro. subst. exfalso. clear - Q_JOIN H4 AT_E MQ_PTC MS.
+                   inv H4. inv Q_JOIN.
+                   destruct wA as (se0 & [se0' m0'] & se1 & [se1' sig'] & se2 & w_cap & w_e).
+                   destruct MQ_PTC as [q1' [Hqr [q1'' [Hqw [qa' [Hqca Hqe]]]]]].
+                   inv Hqr. inv Hqw. simpl in H0. destruct H0.
+                   inv Hqca. inv Hqe. destruct H2 as [PCN Hme].
+                   subst tvf targs.
+                   destruct MS as [EQ1 [EQ2 [MSE EQ3]]].
+                   inv EQ1. inv EQ2. inv EQ3. inv H2. inv H3. simpl in H0.
+                   inv MSE. inv H7. generalize (H0 PC). intro. rewrite <- H4 in H2. inv H2. inv H20.
+                   rewrite RS_PC in H14. inv H14.
+                   inv H5. exploit mge_symb; eauto. intro. apply H2 in FINDPTC.
+                   apply Genv.find_invert_symbol in FINDPTC.
+                   apply Genv.find_invert_symbol in FINDPTJ.
+                   unfold se in FINDPTC.
+                   setoid_rewrite FINDPTC in FINDPTJ. inv FINDPTJ.
+                -- inv DetC. exfalso. eapply sd_big_final_noext; eauto.
+          }
+          destruct H as [rc_ptc [qc_str [s1'k [CREATE AFTER]]]].
           exploit trans_pthread_create__start_routine; eauto.
-          intros (gw & wA'c & ra_ptc & qa_str & PTR_TO_STR_ASM & ACCGTRANS & ACCG & ACCE &NTID & MR_PTC & MQ_STR &  MS_NT & WORLDS).
+          intros (gw & wA'c & ACCGTRANS & ACCG & ACCE &NTID & MR_PTC & MQ_STR &  MS_NT & WORLDS).
           inv WORLDS.
           set (wA'c_injp := {|
                         cajw_injp := injpw j (Mem.yield m' id P1) tm''' Hm2;
                         cajw_sg := start_routine_sig;
                         cajw_rs := ((rs # PC <- (rs RSI)) # RDI <- (rs RDX)) # RSP <- (Vptr sp Ptrofs.zero) |} ).
           assert (wP = wPcur). congruence. subst wP.
-          exploit MR; eauto. intros (li' & lsa' & AFTERa & MSla).
+          exploit MR; eauto. intro Hrex. inv Hrex.
+          exploit bsim_match_cont_match; eauto.
+          intros [lsa' [AFTERc [li' MSlc]]].
           specialize (get_nth_set (cur-1) i li li' GETi).
           intros (i' & SETi' & GETi' & OTHERi).
           set (i'' := i' ++ (li::nil)).
           (** li for new thread is useless, also no effect? hopefully*)
           exists i''. eexists. split.
-          -- left. eapply plus_one.
-             destruct qa_ptc.
-             eapply step_thread_create; eauto. 
+          -- left. eapply plus_right. eapply local_star_c; eauto.
+             eapply CMulti.step_thread_create; eauto. unfoldC. apply NatMap.gss. eauto.
           -- (*match_states*)
              simpl.
              set (worlds' := NatMap.set next (Some wA'c) worldsB).
@@ -2138,16 +1213,17 @@ Admitted
              simpl. lia.
              eauto. eauto. simpl. unfold get_cqv. simpl.
              intros. destruct (Nat.eq_dec 1 cur). subst.
-               rewrite NatMap.gss. congruence.
-               rewrite NatMap.gso; eauto. 
-               rewrite NatMap.gso. eauto. lia.
+             rewrite NatMap.gss. congruence.
+             rewrite NatMap.gso; eauto. 
+             rewrite NatMap.gso. eauto. simpl.
+             rewrite NatMap.gso. eauto. lia. lia.
              instantiate (6:= worlds'). unfold worlds'.
              rewrite NatMap.gso. eauto. lia.
-             intros. unfold worlds' in H7. destruct (Nat.eq_dec n next).
-             subst. rewrite NatMap.gss in H7. inv H7. simpl.
+             intros. unfold worlds' in H8. destruct (Nat.eq_dec n next).
+             subst. rewrite NatMap.gss in H8. inv H8. simpl.
              erewrite w_compcert_sig_eq. rewrite <- H. simpl. split; reflexivity.
              eauto.
-             rewrite NatMap.gso in H7. eauto. eauto.
+             rewrite NatMap.gso in H8. eauto. eauto.
              simpl. instantiate (2:= worldsP').
              unfold worldsP'. rewrite NatMap.gso. rewrite NatMap.gss. reflexivity. lia.
              simpl.
@@ -2161,28 +1237,28 @@ Admitted
                unfold worldsP'.
                exploit FIND_TID. eauto. intro TIDC.
                intros. destruct (Nat.eq_dec n next).
-               - subst. rewrite NatMap.gss in H6.
+               - subst. rewrite NatMap.gss in H7.
                  assert (WEQ: get wA'c = wp). congruence.
                  unfold gw_tid. simpl. split.
                  rewrite <- WEQ. rewrite w_get_injp_eq. rewrite <- H. simpl.
                  destruct CUR_INJP_TID as [C D].
                  apply gw_acci_nexttid in APP. rewrite <- D in APP.
-                 rewrite <- APP. unfold gw_nexttid. rewrite w_get_injp_eq. rewrite <- H4.
+                 rewrite <- APP. unfold gw_nexttid. rewrite w_get_injp_eq. rewrite <- H6.
                  simpl. inv Htc1. reflexivity. lia.
-               - destruct TIDC as [X Y]. rewrite NatMap.gso in H6. 2:lia.
+               - destruct TIDC as [X Y]. rewrite NatMap.gso in H7. 2:lia.
                  destruct (Nat.eq_dec n cur).
                  +
-                   subst. rewrite NatMap.gss in H6. inv H6.
+                   subst. rewrite NatMap.gss in H7. inv H7.
                    split. apply gw_acce_tid in ACCE. rewrite ACCE.
                    apply gw_acci_tid in APP. rewrite APP. reflexivity.
                    simpl. lia.
-                 + rewrite NatMap.gso in H6. inv H6.
+                 + rewrite NatMap.gso in H7. inv H7.
                    assert (injp_tid (injp_gw_compcert wp) = n).
                    { eapply FIND_TID; eauto. }
-                   split. eauto. simpl. rewrite <- H6.
+                   split. eauto. simpl. rewrite <- H7.
                    exploit FIND_TID; eauto. intros [Z1 Z2]. lia. eauto.
              }
-             simpl. eauto. simpl. intros. destruct (Nat.eq_dec n next).
+             simpl. eauto. simpl. eauto. simpl. intros. destruct (Nat.eq_dec n next).
              ++ (* the new thread *) subst.
                 instantiate (1:= NatMap.set (Datatypes.length i'') None worldsA).
                exists wA'c. exists None. eexists. eexists. eexists. eexists. repeat apply conj.
@@ -2198,16 +1274,16 @@ Admitted
                ** rewrite NatMap.gso. rewrite NatMap.gss. reflexivity. lia.
                ** rewrite NatMap.gso. rewrite NatMap.gss. reflexivity. lia.
                ** rewrite NatMap.gss. reflexivity.
-               ** destruct q_str, qa_str.
+               ** destruct q_str, qc_str.
                   econstructor. 
-                  unfold get_cqv, get_query. eauto.
-                  inv H3. reflexivity.
+                  unfold get_cqv, get_query. eauto. simpl. 
+                  inv CREATE. reflexivity.
                **
                unfold worldsP'. rewrite NatMap.gss. reflexivity.
                ** intros. eauto.
              ++ destruct (Nat.eq_dec n cur).
           * (*the executing thread *) subst.
-            exists wB, None, gw, (CMulti.Local OpenC ls'),(Local OpenA lsa'), li'.
+            exists wB, None, gw, (CMulti.Local OpenC lsa'),(Local OpenA ls'), li'.
             repeat apply conj; eauto.
             unfold worlds'. rewrite NatMap.gso. eauto. lia.
             unfold i''. rewrite nth_error_app1. eauto. unfold i'' in CUR_VALID.
@@ -2229,79 +1305,43 @@ Admitted
             repeat rewrite NatMap.gso; eauto.
             repeat rewrite NatMap.gso; eauto. congruence.
             unfold worldsP'. repeat rewrite NatMap.gso; eauto.
-            intros. specialize (J H7).
+            intros. specialize (J H8).
             exploit gw_accg_acci_accg; eauto.
             eapply match_query_wt; eauto.
-        + (** step_switch *)
-          rename s1' into s1''. rename s' into s1'.
-          exploit substep_switch_out; eauto.
-          intros (s2' & tm' & ttm' & worldsP & wpc & f & Hme' & Hmj' & A & B & C & D & E& F).
-          exploit substep_switch_in; eauto.
-          intros (s2'' & i' & X & Y).
-          exists i', s2''. split. left. eapply plus_one. eapply step_switch; eauto. eauto.
+        + (* switch *)
+          admit.
+   Admitted.
+   
+   Lemma Concur_BSimP : Closed.bsim_properties ConcurC ConcurA global_index global_order match_states.
+      constructor. auto.
+      - eapply global_index_wf.
+      - eapply concur_initial_states_exist; eauto.
+      - eapply concur_initial_states.
+      - eapply concur_final_states.
+      - eapply concur_progress.
+      - eapply concur_step.
       - intros. f_equal. simpl. unfold initial_se, CMulti.initial_se. congruence.
-Qed.
+   Qed.
 
-   Theorem Concur_Sim : Closed.forward_simulation ConcurC ConcurA.
-   Proof. econstructor. eapply Concur_FSimP. Qed.
+   Theorem Concur_Sim : Closed.backward_simulation ConcurC ConcurA.
+   Proof. econstructor. eapply Concur_BSimP. Qed.
 
-   Theorem Concur_BSim :
-     determinate OpenA -> receptive OpenC ->
-     Closed.backward_simulation ConcurC ConcurA.
-   Proof.
-     intros DetA' RecC'.
-     generalize (DetA' (Closed.symbolenv (ConcurA))). intro DetA.
-     generalize (RecC' (Closed.symbolenv (ConcurC))). intro RecC.
-     generalize Concur_FSimP. intro FSIMP.
-     econstructor. instantiate (1:= match_states). instantiate (1:= global_order).
-     inv FSIMP.
-     constructor.
-     - eapply global_index_wf.
-     - intros. exploit fsim_match_initial_states; eauto.
-       intros [i [si [I M]]]. eauto.
-     - intros. exploit fsim_match_initial_states; eauto.
-       intros [i [s2' [I M]]]. inv DetA.
-       inv H0. inv I. rewrite H1 in H0. inv H0.
-       rewrite H2 in H4. inv H4. rewrite H3 in H6. inv H6.
-       exploit sd_initial_determ. 
-       apply H5. apply H8. intro. subst. eauto.
-     - intros. red in H0.
-       exploit H0. eapply star_refl. intros [[r1 A] | B].
-       + exists s1. split. eapply star_refl. exploit fsim_match_final_states; eauto.
-       intro. admit.
-       + admit.     (** Determinate*)                
-     - intros. red in H0.
-       exploit H0. eapply star_refl. intros [[r1 A] | [t [s1' B]]].
-       + left. exploit fsim_match_final_states; eauto.
-       + right. exploit fsim_simulation; eauto.
-         intros. destruct H1 as [i' [s2' [[P|S] M]]].
-         clear H0. inv P. eauto.
-         admit. (*stuttering*)
-     - intros. red in H1.
-       exploit H1. eapply star_refl. intros [[r1 A] | [t' [s1' B]]]; clear H1.
-       + exploit fsim_match_final_states; eauto. intro FA.
-         exfalso. admit. (*determ*)
-       + exploit fsim_simulation; eauto.
-         intros [i' [s2'' [[P|S]M]]].
-         -- (** We have to change [match_state] *)
-           admit.
-         -- admit.
-     - intros. f_equal. simpl. unfold initial_se, CMulti.initial_se. congruence.
-   Abort.
        
-  End FSIM.
+  End BSIM.
 
-  Lemma SIM : GS.forward_simulation cc_compcert OpenC OpenA ->
-    Closed.forward_simulation ConcurC ConcurA.
+  Definition final_noundef (lts : semantics li_c li_c) : Prop :=
+   forall s v m se,
+        Smallstep.final_state (lts se) s (cr v m) ->
+        v <> Vundef.
+    
+    
+  Lemma BSIM : GS.backward_simulation cc_compcert OpenC OpenA ->
+               final_noundef OpenC ->
+               determinate_big OpenC ->
+               Closed.backward_simulation ConcurC ConcurA.
   Proof.
-    intro. inv H. inv X. eapply Concur_Sim; eauto.
+    intros. inv H. inv X. eapply Concur_Sim; eauto.
   Qed.
 
 End ConcurSim.
 
-Theorem Opensim_to_Globalsim : forall OpenC OpenA,
-    GS.forward_simulation cc_compcert OpenC OpenA ->
-    Closed.forward_simulation (Concur_sem_c OpenC) (Concur_sem_asm OpenA).
-Proof.
-  intros. eapply SIM; eauto.
-Qed.
